Weidenbach_Book/CDCL_NOT.thy
@@ -229,7 +229,7 @@ locale dpll_state =
     clauses_tl_trail[simp]: "\<And>st. clauses (tl_trail st) = clauses st" and
     clauses_add_cls\<^sub>N\<^sub>O\<^sub>T[simp]:
       "\<And>st C. no_dup (trail st) \<Longrightarrow> clauses (add_cls\<^sub>N\<^sub>O\<^sub>T C st) = {#C#} + clauses st" and
-    clauses_remove_cls\<^sub>N\<^sub>O\<^sub>T[simp]: "\<And>st C. clauses (remove_cls\<^sub>N\<^sub>O\<^sub>T C st) = remove_mset C (clauses st)"
+    clauses_remove_cls\<^sub>N\<^sub>O\<^sub>T[simp]: "\<And>st C. clauses (remove_cls\<^sub>N\<^sub>O\<^sub>T C st) = removeAll_mset C (clauses st)"
 begin
 
 function reduce_trail_to\<^sub>N\<^sub>O\<^sub>T :: "'a list \<Rightarrow> 'st \<Rightarrow> 'st" where
