Weidenbach_Book/CDCL_W_Merge_Implementation.thy
@@ -1,0 +1,2242 @@
+theory CDCL_W_Merge_Implementation
+imports DPLL_CDCL_W_Implementation CDCL_WNOT
+begin
+
+notation image_mset (infixr "`#" 90)
+
+type_synonym 'a cdcl\<^sub>W_mark = "'a clause"
+type_synonym cdcl\<^sub>W_marked_level = nat
+
+type_synonym 'v cdcl\<^sub>W_marked_lit = "('v, cdcl\<^sub>W_marked_level, 'v cdcl\<^sub>W_mark) marked_lit"
+type_synonym 'v cdcl\<^sub>W_marked_lits = "('v, cdcl\<^sub>W_marked_level, 'v cdcl\<^sub>W_mark) marked_lits"
+type_synonym 'v cdcl\<^sub>W_state =
+  "'v cdcl\<^sub>W_marked_lits \<times> 'v clauses \<times> 'v clauses \<times> nat \<times> 'v clause option"
+
+abbreviation trail :: "'a \<times> 'b \<times> 'c \<times> 'd \<times> 'e \<Rightarrow> 'a" where
+"trail \<equiv> (\<lambda>(M, _). M)"
+
+abbreviation cons_trail :: "'a \<Rightarrow> 'a list \<times> 'b \<times> 'c \<times> 'd \<times> 'e \<Rightarrow> 'a list \<times> 'b \<times> 'c \<times> 'd \<times> 'e"
+  where
+"cons_trail \<equiv> (\<lambda>L (M, S). (L#M, S))"
+
+abbreviation tl_trail :: "'a list \<times> 'b \<times> 'c \<times> 'd \<times> 'e \<Rightarrow> 'a list \<times> 'b \<times> 'c \<times> 'd \<times> 'e" where
+"tl_trail \<equiv> (\<lambda>(M, S). (tl M, S))"
+
+abbreviation clss :: "'a \<times> 'b \<times> 'c \<times> 'd \<times> 'e \<Rightarrow> 'b" where
+"clss \<equiv> \<lambda>(M, N, _). N"
+
+abbreviation learned_clss :: "'a \<times> 'b \<times> 'c \<times> 'd \<times> 'e \<Rightarrow> 'c" where
+"learned_clss \<equiv> \<lambda>(M, N, U, _). U"
+
+abbreviation backtrack_lvl :: "'a \<times> 'b \<times> 'c \<times> 'd \<times> 'e \<Rightarrow> 'd" where
+"backtrack_lvl \<equiv> \<lambda>(M, N, U, k, _). k"
+
+abbreviation update_backtrack_lvl :: "'d \<Rightarrow> 'a \<times> 'b \<times> 'c \<times> 'd \<times> 'e \<Rightarrow> 'a \<times> 'b \<times> 'c \<times> 'd \<times> 'e"
+  where
+"update_backtrack_lvl \<equiv> \<lambda>k (M, N, U, _, S).  (M, N, U, k, S)"
+
+abbreviation conflicting :: "'a \<times> 'b \<times> 'c \<times> 'd \<times> 'e \<Rightarrow> 'e" where
+"conflicting \<equiv> \<lambda>(M, N, U, k, D). D"
+
+abbreviation update_conflicting :: "'e \<Rightarrow> 'a \<times> 'b \<times> 'c \<times> 'd \<times> 'e \<Rightarrow> 'a \<times> 'b \<times> 'c \<times> 'd \<times> 'e"
+  where
+"update_conflicting \<equiv> \<lambda>S (M, N, U, k, _).  (M, N, U, k, S)"
+
+abbreviation "S0_cdcl\<^sub>W N \<equiv> (([], N, {#}, 0, None):: 'v cdcl\<^sub>W_state)"
+
+abbreviation add_learned_cls where
+"add_learned_cls \<equiv> \<lambda>C (M, N, U, S). (M, N, {#C#} + U, S)"
+
+abbreviation remove_cls where
+"remove_cls \<equiv> \<lambda>C (M, N, U, S). (M, remove_mset C N, remove_mset C U, S)"
+
+lemma trail_conv: "trail (M, N, U, k, D) = M" and
+  clauses_conv: "clss (M, N, U, k, D) = N" and
+  learned_clss_conv: "learned_clss (M, N, U, k, D) = U" and
+  conflicting_conv: "conflicting (M, N, U, k, D) = D" and
+  backtrack_lvl_conv: "backtrack_lvl (M, N, U, k, D) = k"
+  by auto
+
+lemma state_conv:
+  "S = (trail S, clss S, learned_clss S, backtrack_lvl S, conflicting S)"
+  by (cases S) auto
+
+
+interpretation state\<^sub>W trail clss learned_clss backtrack_lvl conflicting
+  "\<lambda>L (M, S). (L # M, S)"
+  "\<lambda>(M, S). (tl M, S)"
+  "\<lambda>C (M, N, S). (M, {#C#} + N, S)"
+  "\<lambda>C (M, N, U, S). (M, N, {#C#} + U, S)"
+  "\<lambda>C (M, N, U, S). (M, remove_mset C N, remove_mset C U, S)"
+  "\<lambda>(k::nat) (M, N, U, _, D). (M, N, U, k, D)"
+  "\<lambda>D (M, N, U, k, _). (M, N, U, k, D)"
+  "\<lambda>N. ([], N, {#}, 0, None)"
+  "\<lambda>(_, N, U, _). ([], N, U, 0, None)"
+  by unfold_locales auto
+
+interpretation cdcl\<^sub>W trail clss learned_clss backtrack_lvl conflicting
+  "\<lambda>L (M, S). (L # M, S)"
+  "\<lambda>(M, S). (tl M, S)"
+  "\<lambda>C (M, N, S). (M, {#C#} + N, S)"
+  "\<lambda>C (M, N, U, S). (M, N, {#C#} + U, S)"
+  "\<lambda>C (M, N, U, S). (M, remove_mset C N, remove_mset C U, S)"
+  "\<lambda>(k::nat) (M, N, U, _, D). (M, N, U, k, D)"
+  "\<lambda>D (M, N, U, k, _). (M, N, U, k, D)"
+  "\<lambda>N. ([], N, {#}, 0, None)"
+  "\<lambda>(_, N, U, _). ([], N, U, 0, None)"
+  by unfold_locales auto
+
+declare clauses_def[simp]
+
+lemma cdcl\<^sub>W_state_eq_equality[iff]: "state_eq S T \<longleftrightarrow> S = T"
+  unfolding state_eq_def by (cases S, cases T) auto
+declare state_simp[simp del]
+
+subsection \<open>CDCL Implementation\<close>
+subsubsection \<open>Definition of the rules\<close>
+paragraph \<open>Types\<close>
+lemma true_clss_remdups[simp]:
+  "I \<Turnstile>s (mset \<circ> remdups) ` N \<longleftrightarrow>  I \<Turnstile>s mset ` N"
+  by (simp add: true_clss_def)
+
+lemma satisfiable_mset_remdups[simp]:
+  "satisfiable ((mset \<circ> remdups) ` N) \<longleftrightarrow> satisfiable (mset ` N)"
+unfolding satisfiable_carac[symmetric] by simp
+
+value "backtrack_split [Marked (Pos (Suc 0)) ()]"
+value "\<exists>C \<in> set [[Pos (Suc 0), Neg (Suc 0)]]. (\<forall>c \<in> set C. -c \<in> lits_of [Marked (Pos (Suc 0)) ()])"
+
+type_synonym cdcl\<^sub>W_state_inv_st = "(nat, nat, nat literal list) marked_lit list \<times>
+  nat literal list list \<times> nat literal list list \<times> nat \<times> nat literal list option"
+
+text \<open>We need some functions to convert between our abstract state @{typ "nat cdcl\<^sub>W_state"} and the
+ concrete state @{typ "cdcl\<^sub>W_state_inv_st"}.\<close>
+
+fun convert :: "('a, 'b, 'c list) marked_lit \<Rightarrow> ('a, 'b, 'c multiset) marked_lit"  where
+"convert (Propagated L C) = Propagated L (mset C)" |
+"convert (Marked K i) = Marked K i"
+
+abbreviation convertC :: "'a list option \<Rightarrow> 'a multiset option"  where
+"convertC \<equiv> map_option mset"
+
+lemma convert_Propagated[elim!]:
+  "convert z = Propagated L C \<Longrightarrow> (\<exists>C'. z = Propagated L C' \<and> C = mset C')"
+  by (cases z) auto
+
+lemma get_rev_level_map_convert:
+  "get_rev_level (map convert M) n x = get_rev_level M n x"
+  by (induction M arbitrary: n rule: marked_lit_list_induct) auto
+
+lemma get_level_map_convert[simp]:
+  "get_level (map convert M) = get_level M"
+  using get_rev_level_map_convert[of "rev M"] by (simp add: rev_map)
+
+lemma get_maximum_level_map_convert[simp]:
+  "get_maximum_level (map convert M) D = get_maximum_level M D"
+  by (induction D)
+     (auto simp add: get_maximum_level_plus)
+
+lemma get_all_levels_of_marked_map_convert[simp]:
+  "get_all_levels_of_marked (map convert M) = (get_all_levels_of_marked M)"
+  by (induction M rule: marked_lit_list_induct) auto
+
+text \<open>Conversion function\<close>
+fun toS :: "cdcl\<^sub>W_state_inv_st \<Rightarrow> nat cdcl\<^sub>W_state" where
+"toS (M, N, U, k, C) = (map convert M, mset (map mset N),  mset (map mset U), k, convertC C)"
+
+text \<open>Definition an abstract type\<close>
+typedef cdcl\<^sub>W_state_inv =  "{S::cdcl\<^sub>W_state_inv_st. cdcl\<^sub>W_all_struct_inv (toS S)}"
+  morphisms rough_state_of state_of
+proof
+  show "([],[], [], 0, None) \<in> {S. cdcl\<^sub>W_all_struct_inv (toS S)}"
+    by (auto simp add: cdcl\<^sub>W_all_struct_inv_def)
+qed
+
+instantiation cdcl\<^sub>W_state_inv :: equal
+begin
+definition equal_cdcl\<^sub>W_state_inv :: "cdcl\<^sub>W_state_inv \<Rightarrow> cdcl\<^sub>W_state_inv \<Rightarrow> bool" where
+ "equal_cdcl\<^sub>W_state_inv S S' = (rough_state_of S = rough_state_of S')"
+instance
+  by standard (simp add: rough_state_of_inject equal_cdcl\<^sub>W_state_inv_def)
+end
+
+lemma lits_of_map_convert[simp]: "lits_of (map convert M) = lits_of M"
+  by (induction M rule: marked_lit_list_induct) simp_all
+
+lemma undefined_lit_map_convert[iff]:
+  "undefined_lit (map convert M) L \<longleftrightarrow> undefined_lit M L"
+  by (auto simp add: Marked_Propagated_in_iff_in_lits_of)
+
+lemma true_annot_map_convert[simp]: "map convert M \<Turnstile>a N \<longleftrightarrow> M \<Turnstile>a N"
+  by (induction M rule: marked_lit_list_induct) (simp_all add: true_annot_def)
+
+lemma true_annots_map_convert[simp]: "map convert M \<Turnstile>as N \<longleftrightarrow> M \<Turnstile>as N"
+  unfolding true_annots_def by auto
+
+lemmas propagateE
+lemma find_first_unit_clause_some_is_propagate:
+  assumes H: "find_first_unit_clause (N @ U) M = Some (L, C)"
+  shows "propagate (toS (M, N, U, k, None)) (toS (Propagated L C # M, N, U, k, None))"
+  using assms
+  by (auto dest!: find_first_unit_clause_some simp add: propagate.simps
+    intro!: exI[of _ "mset C - {#L#}"])
+
+subsubsection \<open>The Transitions\<close>
+paragraph \<open>Propagate\<close>
+definition do_propagate_step where
+"do_propagate_step S =
+  (case S of
+    (M, N, U, k, None) \<Rightarrow>
+      (case find_first_unit_clause (N @ U) M of
+        Some (L, C) \<Rightarrow> (Propagated L C # M, N, U, k, None)
+      | None \<Rightarrow> (M, N, U, k, None))
+  | S \<Rightarrow> S)"
+
+lemma do_propgate_step:
+  "do_propagate_step S \<noteq> S \<Longrightarrow> propagate (toS S) (toS (do_propagate_step S))"
+  apply (cases S, cases "conflicting S")
+  using find_first_unit_clause_some_is_propagate[of "clss S" "learned_clss S" "trail S" _ _
+    "backtrack_lvl S"]
+  by (auto simp add: do_propagate_step_def split: option.splits)
+
+lemma do_propagate_step_option[simp]:
+  "conflicting S \<noteq> None \<Longrightarrow> do_propagate_step S = S"
+  unfolding do_propagate_step_def by (cases S, cases "conflicting S") auto
+
+lemma do_propagate_step_no_step:
+  assumes dist: "\<forall>c\<in>set (clss S @ learned_clss S). distinct c" and
+  prop_step: "do_propagate_step S = S"
+  shows "no_step propagate (toS S)"
+proof (standard, standard)
+  fix T
+  assume "propagate (toS S) T"
+  then obtain M N U k C L where
+    toSS: "toS S = (M, N, U, k, None)" and
+    T: "T = (Propagated L (C + {#L#}) # M, N, U, k, None)" and
+    MC: "M \<Turnstile>as CNot C" and
+    undef: "undefined_lit M L" and
+    CL: "C + {#L#} \<in># N + U"
+    apply - by (cases "toS S") auto
+  let ?M = "trail S"
+  let ?N = "clss S"
+  let ?U = "learned_clss S"
+  let ?k = "backtrack_lvl S"
+  let ?D = "None"
+  have S: "S = (?M, ?N, ?U, ?k, ?D)"
+    using toSS by (cases S, cases "conflicting S") simp_all
+  have S: "toS S = toS (?M, ?N, ?U, ?k, ?D)"
+    unfolding S[symmetric] by simp
+
+  have
+    M: "M = map convert ?M" and
+    N: "N = mset (map mset ?N)" and
+    U: "U = mset (map mset ?U)"
+    using toSS[unfolded S] by auto
+
+  obtain D where
+    DCL: "mset D = C + {#L#}" and
+    D: "D \<in> set (?N @ ?U)"
+    using CL unfolding N U by auto
+  obtain C' L' where
+    setD: "set D = set (L' # C')" and
+    C': "mset C' = C" and
+    L: "L = L'"
+    using DCL by (metis ex_mset mset.simps(2) mset_eq_setD)
+  have "find_first_unit_clause (?N @ ?U) ?M \<noteq> None"
+    apply (rule dist find_first_unit_clause_none[of D "?N @ ?U" ?M L, OF _ D ])
+       using D assms(1) apply auto[1]
+      using MC setD DCL M MC unfolding C'[symmetric] apply auto[1]
+     using M undef apply auto[1]
+    unfolding setD L by auto
+  then show False using prop_step S unfolding do_propagate_step_def by (cases S) auto
+qed
+
+paragraph \<open>Conflict\<close>
+fun find_conflict where
+"find_conflict M [] = None" |
+"find_conflict M (N # Ns) = (if (\<forall>c \<in> set N. -c \<in> lits_of M) then Some N else find_conflict M Ns)"
+
+lemma find_conflict_Some:
+  "find_conflict M Ns = Some N \<Longrightarrow> N \<in> set Ns \<and> M \<Turnstile>as CNot (mset N)"
+  by (induction Ns rule: find_conflict.induct)
+     (auto split: if_split_asm)
+
+lemma find_conflict_None:
+  "find_conflict M Ns = None \<longleftrightarrow> (\<forall>N \<in> set Ns. \<not>M \<Turnstile>as CNot (mset N))"
+  by (induction Ns) auto
+
+lemma find_conflict_None_no_confl:
+  "find_conflict M (N@U) = None \<longleftrightarrow> no_step conflict (toS (M, N, U, k, None))"
+  by (auto simp add: find_conflict_None conflict.simps)
+
+definition do_conflict_step where
+"do_conflict_step S =
+  (case S of
+    (M, N, U, k, None) \<Rightarrow>
+      (case find_conflict M (N @ U) of
+        Some a \<Rightarrow> (M, N, U, k, Some a)
+      | None \<Rightarrow> (M, N, U, k, None))
+  | S \<Rightarrow> S)"
+
+lemma do_conflict_step:
+  "do_conflict_step S \<noteq> S \<Longrightarrow> conflict (toS S) (toS (do_conflict_step S))"
+  apply (cases S, cases "conflicting S")
+  unfolding conflict.simps do_conflict_step_def
+  by (auto dest!:find_conflict_Some split: option.splits)
+
+lemma do_conflict_step_no_step:
+  "do_conflict_step S = S \<Longrightarrow> no_step conflict (toS S)"
+  apply (cases S, cases "conflicting S")
+  unfolding do_conflict_step_def
+  using find_conflict_None_no_confl[of "trail S" "clss S" "learned_clss S"
+      "backtrack_lvl S"]
+  by (auto split: option.splits)
+
+lemma do_conflict_step_option[simp]:
+  "conflicting S \<noteq> None \<Longrightarrow> do_conflict_step S = S"
+  unfolding do_conflict_step_def by (cases S, cases "conflicting S") auto
+
+lemma do_conflict_step_conflicting[dest]:
+  "do_conflict_step S \<noteq> S \<Longrightarrow> conflicting (do_conflict_step S) \<noteq> None"
+  unfolding do_conflict_step_def by (cases S, cases "conflicting S") (auto split: option.splits)
+
+definition do_cp_step where
+"do_cp_step S =
+  (do_propagate_step o do_conflict_step) S"
+
+lemma cp_step_is_cdcl\<^sub>W_cp:
+  assumes H: "do_cp_step S \<noteq> S"
+  shows "cdcl\<^sub>W_cp (toS S) (toS (do_cp_step S))"
+proof -
+  show ?thesis
+  proof (cases "do_conflict_step S \<noteq> S")
+    case True
+    then show ?thesis
+      by (auto simp add: do_conflict_step do_conflict_step_conflicting do_cp_step_def)
+  next
+    case False
+    then have confl[simp]: "do_conflict_step S = S" by simp
+    show ?thesis
+      proof (cases "do_propagate_step S = S")
+        case True
+        then show ?thesis
+        using H by (simp add: do_cp_step_def)
+      next
+        case False
+        let ?S = "toS S"
+        let ?T = "toS (do_propagate_step S)"
+        let ?U = "toS (do_conflict_step (do_propagate_step S))"
+        have propa: "propagate (toS S) ?T" using False do_propgate_step by blast
+        moreover have ns: "no_step conflict (toS S)" using confl do_conflict_step_no_step by blast
+        ultimately show ?thesis
+          using cdcl\<^sub>W_cp.intros(2)[of ?S ?T] confl unfolding do_cp_step_def by auto
+      qed
+  qed
+qed
+
+lemma do_cp_step_eq_no_prop_no_confl:
+  "do_cp_step S = S \<Longrightarrow> do_conflict_step S = S \<and> do_propagate_step S = S"
+  by (cases S, cases "conflicting S")
+    (auto simp add: do_conflict_step_def do_propagate_step_def do_cp_step_def split: option.splits)
+
+lemma no_cdcl\<^sub>W_cp_iff_no_propagate_no_conflict:
+  "no_step cdcl\<^sub>W_cp S \<longleftrightarrow> no_step propagate S \<and> no_step conflict S"
+  by (auto simp: cdcl\<^sub>W_cp.simps)
+
+lemma do_cp_step_eq_no_step:
+  assumes H: "do_cp_step S = S" and "\<forall>c \<in> set (clss S @ learned_clss S). distinct c"
+  shows "no_step cdcl\<^sub>W_cp (toS S)"
+  unfolding no_cdcl\<^sub>W_cp_iff_no_propagate_no_conflict
+  using assms apply (cases S, cases "conflicting S")
+  using do_propagate_step_no_step[of S]
+  by (auto dest!: do_cp_step_eq_no_prop_no_confl[simplified] do_conflict_step_no_step
+    split: option.splits)
+
+lemma cdcl\<^sub>W_cp_cdcl\<^sub>W_st: "cdcl\<^sub>W_cp S S' \<Longrightarrow> cdcl\<^sub>W\<^sup>*\<^sup>* S S'"
+  by (simp add: cdcl\<^sub>W_cp_tranclp_cdcl\<^sub>W tranclp_into_rtranclp)
+
+lemma cdcl\<^sub>W_cp_wf_all_inv:
+  "wf {(S', S::'v::linorder cdcl\<^sub>W_state). cdcl\<^sub>W_all_struct_inv S \<and> cdcl\<^sub>W_cp S S'}"
+  (is "wf ?R")
+proof (rule wf_bounded_measure[of _ "\<lambda>S. card (atms_of_mm (clss S))+1"
+    "\<lambda>S. length (trail S) + (if conflicting S = None then 0 else 1)"], goal_cases)
+  case (1 S S')
+  then have "cdcl\<^sub>W_all_struct_inv S" and "cdcl\<^sub>W_cp S S'" by auto
+  moreover then have "cdcl\<^sub>W_all_struct_inv S'"
+    using rtranclp_cdcl\<^sub>W_all_struct_inv_inv cdcl\<^sub>W_cp_cdcl\<^sub>W_st by blast
+  ultimately show ?case
+    by (auto simp:cdcl\<^sub>W_cp.simps elim!: conflictE propagateE
+      dest: length_model_le_vars_all_inv)
+qed
+
+lemma cdcl\<^sub>W_all_struct_inv_rough_state[simp]: "cdcl\<^sub>W_all_struct_inv (toS (rough_state_of S))"
+  using rough_state_of by auto
+
+lemma [simp]: "cdcl\<^sub>W_all_struct_inv (toS S) \<Longrightarrow> rough_state_of (state_of S) = S"
+  by (simp add: state_of_inverse)
+
+lemma rough_state_of_state_of_do_cp_step[simp]:
+  "rough_state_of (state_of (do_cp_step (rough_state_of S))) = do_cp_step (rough_state_of S)"
+proof -
+  have "cdcl\<^sub>W_all_struct_inv (toS (do_cp_step (rough_state_of S)))"
+    apply (cases "do_cp_step (rough_state_of S) = (rough_state_of S)")
+      apply simp
+    using cp_step_is_cdcl\<^sub>W_cp[of "rough_state_of S"] cdcl\<^sub>W_all_struct_inv_rough_state[of S]
+    cdcl\<^sub>W_cp_cdcl\<^sub>W_st rtranclp_cdcl\<^sub>W_all_struct_inv_inv by blast
+  then show ?thesis by auto
+qed
+
+paragraph \<open>Skip\<close>
+fun do_skip_step :: "cdcl\<^sub>W_state_inv_st \<Rightarrow> cdcl\<^sub>W_state_inv_st" where
+"do_skip_step (Propagated L C # Ls,N,U,k, Some D) =
+  (if -L \<notin> set D \<and> D \<noteq> []
+  then (Ls, N, U, k, Some D)
+  else (Propagated L C #Ls, N, U, k, Some D))" |
+"do_skip_step S = S"
+
+lemma do_skip_step:
+  "do_skip_step S \<noteq> S \<Longrightarrow> skip (toS S) (toS (do_skip_step S))"
+  apply (induction S rule: do_skip_step.induct)
+  by (auto simp add: skip.simps)
+
+lemma do_skip_step_no:
+  "do_skip_step S = S \<Longrightarrow> no_step skip (toS S)"
+  by (induction S rule: do_skip_step.induct)
+     (auto simp add: other split: if_split_asm)
+
+lemma do_skip_step_trail_is_None[iff]:
+  "do_skip_step S = (a, b, c, d, None) \<longleftrightarrow> S = (a, b, c, d, None)"
+  by (cases S rule: do_skip_step.cases) auto
+
+paragraph \<open>Resolve\<close>
+fun maximum_level_code:: "'a literal list \<Rightarrow> ('a, nat, 'a literal list) marked_lit list \<Rightarrow> nat"
+  where
+"maximum_level_code [] _ = 0" |
+"maximum_level_code (L # Ls) M = max (get_level M L) (maximum_level_code Ls M)"
+
+lemma maximum_level_code_eq_get_maximum_level[code, simp]:
+  "maximum_level_code D M = get_maximum_level M (mset D)"
+  by (induction D) (auto simp add: get_maximum_level_plus)
+
+fun do_resolve_step :: "cdcl\<^sub>W_state_inv_st \<Rightarrow> cdcl\<^sub>W_state_inv_st" where
+"do_resolve_step (Propagated L C # Ls, N, U, k, Some D) =
+  (if -L \<in> set D \<and> maximum_level_code (remove1 (-L) D) (Propagated L C # Ls) = k
+  then (Ls, N, U, k, Some (remdups (remove1 L C @ remove1 (-L) D)))
+  else (Propagated L C # Ls, N, U, k, Some D))" |
+"do_resolve_step S = S"
+
+lemma do_resolve_step:
+  "cdcl\<^sub>W_all_struct_inv (toS S) \<Longrightarrow> do_resolve_step S \<noteq> S
+  \<Longrightarrow> resolve (toS S) (toS (do_resolve_step S))"
+proof (induction S rule: do_resolve_step.induct)
+  case (1 L C M N U k D)
+  then have
+    "- L \<in> set D" and
+    M: "maximum_level_code (remove1 (-L) D) (Propagated L C # M) = k"
+    by (cases "mset D - {#- L#} = {#}",
+        auto dest!: get_maximum_level_exists_lit_of_max_level[of _ "Propagated L C # M"]
+        split: if_split_asm)+
+  have "every_mark_is_a_conflict (toS (Propagated L C # M, N, U, k, Some D))"
+    using 1(1) unfolding cdcl\<^sub>W_all_struct_inv_def cdcl\<^sub>W_conflicting_def by fast
+  then have "L \<in> set C" by fastforce
+  then obtain C' where C: "mset C = C' + {#L#}"
+    by (metis add.commute in_multiset_in_set insert_DiffM)
+  obtain D' where D: "mset D = D' + {#-L#}"
+    using \<open>- L \<in> set D\<close> by (metis add.commute in_multiset_in_set insert_DiffM)
+  have D'L:  "D' + {#- L#} - {#-L#} = D'" by (auto simp add: multiset_eq_iff)
+
+  have CL: "mset C - {#L#} + {#L#} = mset C" using \<open>L \<in> set C\<close> by (auto simp add: multiset_eq_iff)
+  have "get_maximum_level (Propagated L (C' + {#L#}) # map convert M) D' = k"
+    using M[simplified] unfolding maximum_level_code_eq_get_maximum_level C[symmetric] CL
+    by (metis D D'L convert.simps(1) get_maximum_level_map_convert list.simps(9))
+  then have
+    "resolve
+       (map convert (Propagated L C # M), mset `# mset N, mset `# mset U, k, Some (mset D))
+       (map convert M, mset `# mset N, mset `# mset U, k,
+         Some (((mset D - {#-L#}) #\<union> (mset C - {#L#}))))"
+    unfolding resolve.simps
+      by (simp add: C D)
+  moreover have
+    "(map convert (Propagated L C # M), mset `# mset N, mset `# mset U, k, Some (mset D))
+     = toS (Propagated L C # M, N, U, k, Some D)"
+    by (auto simp: mset_map)
+  moreover
+    have "distinct_mset (mset C)" and "distinct_mset (mset D)"
+      using \<open>cdcl\<^sub>W_all_struct_inv (toS (Propagated L C # M, N, U, k, Some D))\<close>
+      unfolding cdcl\<^sub>W_all_struct_inv_def distinct_cdcl\<^sub>W_state_def
+      by auto
+    then have "(mset C - {#L#}) #\<union> (mset D - {#- L#}) =
+      remdups_mset (mset C - {#L#} + (mset D - {#- L#}))"
+      by (auto simp: distinct_mset_rempdups_union_mset)
+    then have "(map convert M, mset `# mset N, mset `# mset U, k,
+    Some ((mset D - {#- L#}) #\<union> (mset C - {#L#})))
+    = toS (do_resolve_step (Propagated L C # M, N, U, k, Some D))"
+    using \<open>- L \<in> set D\<close> M by (auto simp:ac_simps mset_map)
+  ultimately show ?case
+    by simp
+qed auto
+
+lemma do_resolve_step_no:
+  "do_resolve_step S = S \<Longrightarrow> no_step resolve (toS S)"
+  apply (cases S; cases "hd (trail S)"; cases "conflicting S")
+  by (auto
+    elim!: resolveE  split: if_split_asm
+    dest!: union_single_eq_member
+    simp del: in_multiset_in_set get_maximum_level_map_convert
+    simp: in_multiset_in_set[symmetric] get_maximum_level_map_convert[symmetric])
+
+
+lemma  rough_state_of_state_of_resolve[simp]:
+  "cdcl\<^sub>W_all_struct_inv (toS S) \<Longrightarrow> rough_state_of (state_of (do_resolve_step S)) = do_resolve_step S"
+  apply (rule state_of_inverse)
+  apply (cases "do_resolve_step S = S")
+   apply simp
+  by (blast dest: other resolve bj do_resolve_step cdcl\<^sub>W_all_struct_inv_inv)
+
+lemma do_resolve_step_trail_is_None[iff]:
+  "do_resolve_step S = (a, b, c, d, None) \<longleftrightarrow> S = (a, b, c, d, None)"
+  by (cases S rule: do_resolve_step.cases) auto
+
+paragraph \<open>Backjumping\<close>
+fun find_level_decomp where
+"find_level_decomp M [] D k = None" |
+"find_level_decomp M (L # Ls) D k =
+  (case (get_level M L, maximum_level_code (D @ Ls) M) of
+    (i, j) \<Rightarrow> if i = k \<and> j < i then Some (L, j) else find_level_decomp M Ls (L#D) k
+  )"
+
+lemma find_level_decomp_some:
+  assumes "find_level_decomp M Ls D k = Some (L, j)"
+  shows "L \<in> set Ls \<and> get_maximum_level M (mset (remove1 L (Ls @ D))) = j \<and> get_level M L = k"
+  using assms
+proof (induction Ls arbitrary: D)
+  case Nil
+  then show ?case by simp
+next
+  case (Cons L' Ls) note IH = this(1) and H = this(2)
+  (* heavily modified sledgehammer proof *)
+  def find \<equiv> "(if get_level M L' \<noteq> k \<or> \<not> get_maximum_level M (mset D + mset Ls) < get_level M L'
+    then find_level_decomp M Ls (L' # D) k
+    else Some (L', get_maximum_level M (mset D + mset Ls)))"
+  have a1: "\<And>D. find_level_decomp M Ls D k = Some (L, j) \<Longrightarrow>
+     L \<in> set Ls \<and> get_maximum_level M (mset Ls + mset D - {#L#}) = j \<and> get_level M L = k"
+    using IH by simp
+  have a2: "find = Some (L, j)"
+    using H unfolding find_def by (auto split: if_split_asm)
+  { assume "Some (L', get_maximum_level M (mset D + mset Ls)) \<noteq> find"
+    then have f3: "L \<in> set Ls" and "get_maximum_level M (mset Ls + mset (L' # D) - {#L#}) = j"
+      using a1 IH a2 unfolding find_def by meson+
+    moreover then have "mset Ls + mset D - {#L#} + {#L'#} = {#L'#} + mset D + (mset Ls - {#L#})"
+      by (auto simp: ac_simps multiset_eq_iff Suc_leI)
+    ultimately have f4: "get_maximum_level M (mset Ls + mset D - {#L#} + {#L'#}) = j"
+      by (metis (no_types) diff_union_single_conv mem_set_multiset_eq mset.simps(2) union_commute)
+  } note f4 = this
+  have "{#L'#} + (mset Ls + mset D) = mset Ls + (mset D + {#L'#})"
+      by (auto simp: ac_simps)
+  then have
+    "(L = L' \<longrightarrow> get_maximum_level M (mset Ls + mset D) = j \<and> get_level M L' = k)" and
+    "(L \<noteq> L' \<longrightarrow> L \<in> set Ls \<and> get_maximum_level M (mset Ls + mset D - {#L#} + {#L'#}) = j \<and>
+      get_level M L = k)"
+    using f4 a2 a1[of "L' # D"] unfolding find_def by (metis (no_types) add_diff_cancel_left'
+      mset.simps(2) option.inject prod.inject union_commute)+
+  then show ?case by simp
+qed
+
+lemma find_level_decomp_none:
+  assumes "find_level_decomp M Ls E k = None" and "mset (L#D) = mset (Ls @ E)"
+  shows "\<not>(L \<in> set Ls \<and> get_maximum_level M (mset D) < k \<and> k = get_level M L)"
+  using assms
+proof (induction Ls arbitrary: E L D)
+  case Nil
+  then show ?case by simp
+next
+  case (Cons L' Ls) note IH = this(1) and find_none = this(2) and LD = this(3)
+  have "mset D + {#L'#} = mset E + (mset Ls + {#L'#})  \<Longrightarrow> mset D = mset E + mset Ls"
+    by (metis add_right_imp_eq union_assoc)
+  then show ?case
+    using find_none IH[of "L' # E" L D] LD by (auto simp add: ac_simps split: if_split_asm)
+qed
+
+fun bt_cut where
+"bt_cut i (Propagated _ _ # Ls) = bt_cut i Ls" |
+"bt_cut i (Marked K k # Ls) = (if k = Suc i then Some (Marked K k # Ls) else bt_cut i Ls)" |
+"bt_cut i [] = None"
+
+lemma bt_cut_some_decomp:
+  "bt_cut i M = Some M' \<Longrightarrow> \<exists>K M2 M1. M = M2 @ M' \<and> M' = Marked K (i+1) # M1"
+  by (induction i M rule: bt_cut.induct) (auto split: if_split_asm)
+
+lemma bt_cut_not_none: "M = M2 @ Marked K (Suc i) # M' \<Longrightarrow> bt_cut i M \<noteq> None"
+  by (induction M2 arbitrary: M rule: marked_lit_list_induct) auto
+
+lemma get_all_marked_decomposition_ex:
+  "\<exists>N. (Marked K (Suc i) # M', N) \<in> set (get_all_marked_decomposition (M2@Marked K (Suc i) # M'))"
+  apply (induction M2 rule: marked_lit_list_induct)
+    apply auto[2]
+  by (rename_tac L m xs,  case_tac "get_all_marked_decomposition (xs @ Marked K (Suc i) # M')")
+  auto
+
+lemma bt_cut_in_get_all_marked_decomposition:
+  "bt_cut i M = Some M' \<Longrightarrow> \<exists>M2. (M', M2) \<in> set (get_all_marked_decomposition M)"
+  by (auto dest!: bt_cut_some_decomp simp add: get_all_marked_decomposition_ex)
+
+fun do_backtrack_step where
+"do_backtrack_step (M, N, U, k, Some D) =
+  (case find_level_decomp M D [] k of
+    None \<Rightarrow> (M, N, U, k, Some D)
+  | Some (L, j) \<Rightarrow>
+    (case bt_cut j M of
+      Some (Marked _ _ # Ls) \<Rightarrow> (Propagated L D # Ls, N, D # U, j, None)
+    | _ \<Rightarrow> (M, N, U, k, Some D))
+  )" |
+"do_backtrack_step S = S"
+
+lemma get_all_marked_decomposition_map_convert:
+  "(get_all_marked_decomposition (map convert M)) =
+    map (\<lambda>(a, b). (map convert a, map convert b)) (get_all_marked_decomposition M)"
+  apply (induction M rule: marked_lit_list_induct)
+    apply simp
+  by (rename_tac L l xs, case_tac "get_all_marked_decomposition xs"; auto)+
+
+lemma do_backtrack_step:
+  assumes
+    db: "do_backtrack_step S \<noteq> S" and
+    inv: "cdcl\<^sub>W_all_struct_inv (toS S)"
+  shows "backtrack (toS S) (toS (do_backtrack_step S))"
+  proof (cases S, cases "conflicting S", goal_cases)
+    case (1 M N U k E)
+    then show ?case using db by auto
+  next
+    case (2 M N U k E C) note S = this(1) and confl = this(2)
+    have E: "E = Some C" using S confl by auto
+
+    obtain L j where fd: "find_level_decomp M C [] k = Some (L, j)"
+      using db unfolding S E  by (cases C) (auto split: if_split_asm option.splits)
+    have "L \<in> set C" and "get_maximum_level M (mset (remove1 L C)) = j" and
+      levL: "get_level M L = k"
+      using find_level_decomp_some[OF fd] by auto
+    obtain C' where C: "mset C = mset C' + {#L#}"
+      using \<open>L \<in> set C\<close> by (metis add.commute ex_mset in_multiset_in_set insert_DiffM)
+    obtain M\<^sub>2 where M\<^sub>2: "bt_cut j M = Some M\<^sub>2"
+      using db fd unfolding S E by (auto split: option.splits)
+    obtain M1 K where M1: "M\<^sub>2 = Marked K (Suc j) # M1"
+      using bt_cut_some_decomp[OF M\<^sub>2] by (cases M\<^sub>2) auto
+    obtain c where c: "M = c @ Marked K (Suc j) # M1"
+       using bt_cut_in_get_all_marked_decomposition[OF M\<^sub>2]
+       unfolding M1 by fastforce
+    have "get_all_levels_of_marked (map convert M) = rev [1..<Suc k]"
+      using inv unfolding cdcl\<^sub>W_all_struct_inv_def cdcl\<^sub>W_M_level_inv_def S by auto
+    from arg_cong[OF this, of "\<lambda>a. Suc j \<in> set a"] have "j \<le> k" unfolding c by auto
+    have max_l_j: "maximum_level_code C' M = j"
+      using db fd M\<^sub>2 C unfolding S E by (auto
+          split: option.splits list.splits marked_lit.splits
+          dest!: find_level_decomp_some)[1]
+    have "get_maximum_level M (mset C) \<ge> k"
+      using \<open>L \<in> set C\<close> get_maximum_level_ge_get_level levL by blast
+    moreover have "get_maximum_level M (mset C) \<le> k"
+      using get_maximum_level_exists_lit_of_max_level[of "mset C" M] inv
+        cdcl\<^sub>W_M_level_inv_get_level_le_backtrack_lvl[of "toS S"]
+      unfolding C cdcl\<^sub>W_all_struct_inv_def S by (auto dest: sym[of "get_level _ _"])
+    ultimately have "get_maximum_level M (mset C) = k" by auto
+
+    obtain M2 where M2: "(M\<^sub>2, M2) \<in> set (get_all_marked_decomposition M)"
+      using bt_cut_in_get_all_marked_decomposition[OF M\<^sub>2] by metis
+    have H: "(reduce_trail_to (map convert M1)
+      (add_learned_cls (mset C' + {#L#})
+        (map convert M, mset (map mset N), mset (map mset U), j, None))) =
+        (map convert M1, mset (map mset N), {#mset C' + {#L#}#} + mset (map mset U), j, None)"
+        apply (subst state_conv[of "reduce_trail_to _ _"])
+      using M2 unfolding M1 by auto
+    have
+      "backtrack
+        (map convert M, mset `# mset N, mset `# mset U, k, Some (mset C))
+        (Propagated L (mset C) # map convert M1, mset `# mset N, mset `# mset U + {#mset C#}, j,
+          None)"
+      apply (rule backtrack_rule)
+             unfolding C apply simp
+            using Set.imageI[of "(M\<^sub>2, M2)" "set (get_all_marked_decomposition M)"
+                             "(\<lambda>(a, b). (map convert a, map convert b))"] M2
+            apply (auto simp: get_all_marked_decomposition_map_convert M1)[1]
+           using max_l_j levL \<open>j \<le> k\<close> apply (simp add: get_maximum_level_plus)
+          using C \<open>get_maximum_level M (mset C) = k\<close> levL apply auto[1]
+         using max_l_j apply simp
+        apply (cases "reduce_trail_to (map convert M1)
+            (add_learned_cls (mset C' + {#L#})
+            (map convert M, mset (map mset N), mset (map mset U), j, None))")
+       using M2 M1 H by (auto simp: ac_simps mset_map)
+    then show ?case
+      using M\<^sub>2 fd unfolding S E M1 by (auto simp: mset_map)
+    obtain M2 where "(M\<^sub>2, M2) \<in> set (get_all_marked_decomposition M)"
+      using bt_cut_in_get_all_marked_decomposition[OF M\<^sub>2] by metis
+qed
+
+lemma do_backtrack_step_no:
+  assumes db: "do_backtrack_step S = S"
+  and inv: "cdcl\<^sub>W_all_struct_inv (toS S)"
+  shows "no_step backtrack (toS S)"
+proof (rule ccontr, cases S, cases "conflicting S", goal_cases)
+  case 1
+  then show ?case using db by (auto split: option.splits)
+next
+  case (2 M N U k E C) note bt = this(1) and S = this(2) and confl = this(3)
+  obtain D L K b z M1 j where
+    levL: "get_level M L = get_maximum_level M (D + {#L#})" and
+    k: "k = get_maximum_level M (D + {#L#})" and
+    j: "j = get_maximum_level M D" and
+    CE: "convertC E = Some (D + {#L#})" and
+    decomp: "(z # M1, b) \<in> set (get_all_marked_decomposition M)" and
+    z: "Marked K (Suc j) = convert z" using bt unfolding S
+      by (auto split: option.splits elim!: backtrackE
+        simp: get_all_marked_decomposition_map_convert)
+  have z: "z = Marked K (Suc j)" using z by (cases z) auto
+  obtain c where c: "M = c @ b @ Marked K (Suc j) # M1"
+    using decomp unfolding z by blast
+  have "get_all_levels_of_marked (map convert M) = rev [1..<Suc k]"
+    using inv unfolding cdcl\<^sub>W_all_struct_inv_def cdcl\<^sub>W_M_level_inv_def S by auto
+  from arg_cong[OF this, of "\<lambda>a. Suc j \<in> set a"] have "k > j" unfolding c by auto
+  obtain C D' where
+    E: "E = Some C" and
+    C: "mset C = mset (L # D')"
+    using CE apply (cases E)
+      apply simp
+    by (metis ex_mset mset.simps(2) option.inject option.simps(9))
+  have D'D: "mset D' = D"
+    using C CE E by auto
+  have "find_level_decomp M C [] k \<noteq> None"
+    apply rule
+    apply (drule find_level_decomp_none[of _ _ _ _ L D'])
+    using C \<open>k > j\<close> mset_eq_setD unfolding k[symmetric] D'D j[symmetric] levL by fastforce+
+  then obtain L' j' where fd_some: "find_level_decomp M C [] k = Some (L', j')"
+    by (cases "find_level_decomp M C [] k") auto
+  have L': "L' = L"
+    proof (rule ccontr)
+      assume "\<not> ?thesis"
+      then have "L' \<in># D"
+        by (metis C D'D fd_some find_level_decomp_some in_multiset_in_set insert_iff list.simps(15))
+      then have "get_level M L' \<le> get_maximum_level M D"
+        using get_maximum_level_ge_get_level by blast
+      then show False using \<open>k > j\<close> j find_level_decomp_some[OF fd_some] by auto
+    qed
+  then have j': "j' = j" using find_level_decomp_some[OF fd_some] j C D'D by auto
+
+  have btc_none: "bt_cut j M \<noteq> None"
+    apply (rule bt_cut_not_none[of M "_ @ _"])
+    using c by simp
+  show ?case using db unfolding S  E
+    by (auto split: option.splits list.splits marked_lit.splits
+      simp add: fd_some  L' j' btc_none
+      dest: bt_cut_some_decomp)
+qed
+
+lemma rough_state_of_state_of_backtrack[simp]:
+  assumes inv: "cdcl\<^sub>W_all_struct_inv (toS S)"
+  shows "rough_state_of (state_of (do_backtrack_step S))= do_backtrack_step S"
+proof (rule state_of_inverse)
+  have f2: "backtrack (toS S) (toS (do_backtrack_step S)) \<or> do_backtrack_step S = S"
+    using do_backtrack_step inv by blast
+  have "\<And>p. \<not> cdcl\<^sub>W_o (toS S) p \<or> cdcl\<^sub>W_all_struct_inv p"
+    using inv cdcl\<^sub>W_all_struct_inv_inv other by blast
+  then have "do_backtrack_step S = S \<or> cdcl\<^sub>W_all_struct_inv (toS (do_backtrack_step S))"
+    using f2 by blast
+  then show "do_backtrack_step S \<in> {S. cdcl\<^sub>W_all_struct_inv (toS S)}"
+    using inv by  fastforce
+qed
+
+paragraph \<open>Decide\<close>
+fun do_decide_step where
+"do_decide_step (M, N, U, k, None) =
+  (case find_first_unused_var N (lits_of M) of
+    None \<Rightarrow> (M, N, U, k, None)
+  | Some L \<Rightarrow> (Marked L (Suc k) # M, N, U, k+1, None))" |
+"do_decide_step S = S"
+
+lemma do_decide_step:
+  "do_decide_step S \<noteq> S \<Longrightarrow> decide (toS S) (toS (do_decide_step S))"
+  apply (cases S, cases "conflicting S")
+  defer
+  apply (auto split: option.splits simp add: decide.simps Marked_Propagated_in_iff_in_lits_of
+          dest: find_first_unused_var_undefined find_first_unused_var_Some
+          intro: atms_of_atms_of_ms_mono)[1]
+proof -
+  fix a :: "(nat, nat, nat literal list) marked_lit list" and
+        b :: "nat literal list list" and  c :: "nat literal list list" and
+        d :: nat and e :: "nat literal list option"
+  {
+    fix a :: "(nat, nat, nat literal list) marked_lit list" and
+        b :: "nat literal list list" and  c :: "nat literal list list" and
+        d :: nat and x2 :: "nat literal" and m :: "nat literal list"
+    assume a1: "m \<in> set b"
+    assume "x2 \<in> set m"
+    then have f2: "atm_of x2 \<in> atms_of (mset m)"
+      by simp
+    have "\<And>f. (f m::nat literal multiset) \<in> f ` set b"
+      using a1 by blast
+    then have "\<And>f. (atms_of (f m)::nat set) \<subseteq> atms_of_ms (f ` set b)"
+     using atms_of_atms_of_ms_mono by blast
+    then have "\<And>n f. (n::nat) \<in> atms_of_ms (f ` set b) \<or> n \<notin> atms_of (f m)"
+      by (meson contra_subsetD)
+    then have "atm_of x2 \<in> atms_of_ms (mset ` set b)"
+      using f2 by blast
+  } note H = this
+  {
+    fix m :: "nat literal list" and x2
+    have "m \<in> set b \<Longrightarrow> x2 \<in> set m \<Longrightarrow> x2 \<notin> lits_of a \<Longrightarrow> - x2 \<notin> lits_of a \<Longrightarrow>
+      \<exists>aa\<in>set b. \<not> atm_of ` set aa \<subseteq> atm_of ` lits_of a"
+      by (meson atm_of_in_atm_of_set_in_uminus contra_subsetD rev_image_eqI)
+  } note H' = this
+
+  assume  "do_decide_step S \<noteq> S" and
+     "S = (a, b, c, d, e)" and
+     "conflicting S = None"
+  then show "decide (toS S) (toS (do_decide_step S))"
+    using H H' by (auto split: option.splits simp: decide.simps Marked_Propagated_in_iff_in_lits_of
+      dest!: find_first_unused_var_Some)
+qed
+
+lemma do_decide_step_no:
+  "do_decide_step S = S \<Longrightarrow> no_step decide (toS S)"
+  by (cases S, cases "conflicting S")
+    (fastforce simp: atms_of_ms_mset_unfold atm_of_eq_atm_of Marked_Propagated_in_iff_in_lits_of
+      split: option.splits)+
+
+lemma rough_state_of_state_of_do_decide_step[simp]:
+  "cdcl\<^sub>W_all_struct_inv (toS S) \<Longrightarrow> rough_state_of (state_of (do_decide_step S)) = do_decide_step S"
+proof (subst state_of_inverse, goal_cases)
+  case 1
+  then show ?case
+    by (cases "do_decide_step S = S")
+      (auto dest: do_decide_step decide other intro: cdcl\<^sub>W_all_struct_inv_inv)
+qed simp
+
+lemma rough_state_of_state_of_do_skip_step[simp]:
+  "cdcl\<^sub>W_all_struct_inv (toS S) \<Longrightarrow> rough_state_of (state_of (do_skip_step S)) = do_skip_step S"
+  apply (subst state_of_inverse, cases "do_skip_step S = S")
+   apply simp
+  by (blast dest: other skip bj do_skip_step cdcl\<^sub>W_all_struct_inv_inv)+
+
+subsubsection \<open>Code generation\<close>
+paragraph \<open>Type definition\<close>
+text \<open>There are two invariants: one while applying conflict and propagate and one for the other
+ rules\<close>
+
+declare rough_state_of_inverse[simp add]
+definition Con where
+  "Con xs = state_of (if cdcl\<^sub>W_all_struct_inv (toS (fst xs, snd xs)) then xs
+  else ([], [], [], 0, None))"
+
+lemma [code abstype]:
+ "Con (rough_state_of S) = S"
+  using rough_state_of[of S] unfolding Con_def by simp
+
+definition do_cp_step' where
+"do_cp_step' S = state_of (do_cp_step (rough_state_of S))"
+
+typedef cdcl\<^sub>W_state_inv_from_init_state = "{S::cdcl\<^sub>W_state_inv_st. cdcl\<^sub>W_all_struct_inv (toS S)
+  \<and> cdcl\<^sub>W_stgy\<^sup>*\<^sup>* (S0_cdcl\<^sub>W (clss (toS S))) (toS S)}"
+  morphisms rough_state_from_init_state_of state_from_init_state_of
+proof
+  show "([],[], [], 0, None) \<in> {S. cdcl\<^sub>W_all_struct_inv (toS S)
+    \<and> cdcl\<^sub>W_stgy\<^sup>*\<^sup>* (S0_cdcl\<^sub>W (clss (toS S))) (toS S)}"
+    by (auto simp add: cdcl\<^sub>W_all_struct_inv_def)
+qed
+
+instantiation cdcl\<^sub>W_state_inv_from_init_state :: equal
+begin
+definition equal_cdcl\<^sub>W_state_inv_from_init_state :: "cdcl\<^sub>W_state_inv_from_init_state \<Rightarrow>
+  cdcl\<^sub>W_state_inv_from_init_state \<Rightarrow> bool" where
+ "equal_cdcl\<^sub>W_state_inv_from_init_state S S' \<longleftrightarrow>
+   (rough_state_from_init_state_of S = rough_state_from_init_state_of S')"
+instance
+  by standard (simp add: rough_state_from_init_state_of_inject
+    equal_cdcl\<^sub>W_state_inv_from_init_state_def)
+end
+
+definition ConI where
+  "ConI S = state_from_init_state_of (if cdcl\<^sub>W_all_struct_inv (toS (fst S, snd S))
+    \<and> cdcl\<^sub>W_stgy\<^sup>*\<^sup>* (S0_cdcl\<^sub>W (clss (toS S))) (toS S) then S else ([], [], [], 0, None))"
+
+lemma [code abstype]:
+  "ConI (rough_state_from_init_state_of S) = S"
+  using rough_state_from_init_state_of[of S] unfolding ConI_def
+  by (simp add: rough_state_from_init_state_of_inverse)
+
+definition id_of_I_to:: "cdcl\<^sub>W_state_inv_from_init_state \<Rightarrow> cdcl\<^sub>W_state_inv" where
+"id_of_I_to S = state_of (rough_state_from_init_state_of S)"
+
+lemma [code abstract]:
+  "rough_state_of (id_of_I_to S) = rough_state_from_init_state_of S"
+  unfolding id_of_I_to_def using rough_state_from_init_state_of by auto
+
+paragraph \<open>Conflict and Propagate\<close>
+function do_full1_cp_step :: "cdcl\<^sub>W_state_inv \<Rightarrow> cdcl\<^sub>W_state_inv" where
+"do_full1_cp_step S =
+  (let S' = do_cp_step' S in
+   if S = S' then S else do_full1_cp_step S')"
+by auto
+termination
+proof (relation "{(T', T). (rough_state_of T', rough_state_of T) \<in> {(S', S).
+  (toS S', toS S) \<in> {(S', S). cdcl\<^sub>W_all_struct_inv S \<and> cdcl\<^sub>W_cp S S'}}}", goal_cases)
+  case 1
+  show ?case
+    using wf_if_measure_f[OF wf_if_measure_f[OF cdcl\<^sub>W_cp_wf_all_inv, of "toS"], of rough_state_of] .
+next
+  case (2 S' S)
+  then show ?case
+    unfolding do_cp_step'_def
+    apply simp
+    by (metis cp_step_is_cdcl\<^sub>W_cp rough_state_of_inverse)
+qed
+
+lemma do_full1_cp_step_fix_point_of_do_full1_cp_step:
+  "do_cp_step(rough_state_of (do_full1_cp_step S)) = (rough_state_of (do_full1_cp_step S))"
+  by (rule do_full1_cp_step.induct[of "\<lambda>S. do_cp_step(rough_state_of (do_full1_cp_step S))
+       = (rough_state_of (do_full1_cp_step S))"])
+    (metis (full_types) do_full1_cp_step.elims rough_state_of_state_of_do_cp_step do_cp_step'_def)
+
+lemma in_clauses_rough_state_of_is_distinct:
+  "c\<in>set (clss (rough_state_of S) @ learned_clss (rough_state_of S)) \<Longrightarrow> distinct c"
+  apply (cases "rough_state_of S")
+  using rough_state_of[of S] by (auto simp add: distinct_mset_set_distinct cdcl\<^sub>W_all_struct_inv_def
+    distinct_cdcl\<^sub>W_state_def)
+
+lemma do_full1_cp_step_full:
+  "full cdcl\<^sub>W_cp (toS (rough_state_of S))
+    (toS (rough_state_of (do_full1_cp_step S)))"
+  unfolding full_def
+proof (rule conjI, induction S rule: do_full1_cp_step.induct)
+  case (1 S)
+  then have f1:
+      "cdcl\<^sub>W_cp\<^sup>*\<^sup>* (toS (do_cp_step (rough_state_of S))) (
+        toS (rough_state_of (do_full1_cp_step (state_of (do_cp_step (rough_state_of S))))))
+      \<or> state_of (do_cp_step (rough_state_of S)) = S"
+    using do_cp_step'_def rough_state_of_state_of_do_cp_step by fastforce
+  have f2: "\<And>c. (if c = state_of (do_cp_step (rough_state_of c))
+       then c else do_full1_cp_step (state_of (do_cp_step (rough_state_of c))))
+     = do_full1_cp_step c"
+    by (metis (full_types) do_cp_step'_def do_full1_cp_step.simps)
+  have f3: "\<not> cdcl\<^sub>W_cp (toS (rough_state_of S)) (toS (do_cp_step (rough_state_of S)))
+    \<or> state_of (do_cp_step (rough_state_of S)) = S
+    \<or> cdcl\<^sub>W_cp\<^sup>+\<^sup>+ (toS (rough_state_of S))
+        (toS (rough_state_of (do_full1_cp_step (state_of (do_cp_step (rough_state_of S))))))"
+    using f1 by (meson rtranclp_into_tranclp2)
+  { assume "do_full1_cp_step S \<noteq> S"
+    then have "do_cp_step (rough_state_of S) = rough_state_of S
+        \<longrightarrow> cdcl\<^sub>W_cp\<^sup>*\<^sup>* (toS (rough_state_of S)) (toS (rough_state_of (do_full1_cp_step S)))
+      \<or> do_cp_step (rough_state_of S) \<noteq> rough_state_of S
+        \<and> state_of (do_cp_step (rough_state_of S)) \<noteq> S"
+      using f2 f1 by (metis (no_types))
+    then have "do_cp_step (rough_state_of S) \<noteq> rough_state_of S
+        \<and> state_of (do_cp_step (rough_state_of S)) \<noteq> S
+      \<or> cdcl\<^sub>W_cp\<^sup>*\<^sup>* (toS (rough_state_of S)) (toS (rough_state_of (do_full1_cp_step S)))"
+      by (metis rough_state_of_state_of_do_cp_step)
+    then have "cdcl\<^sub>W_cp\<^sup>*\<^sup>* (toS (rough_state_of S)) (toS (rough_state_of (do_full1_cp_step S)))"
+      using f3 f2 by (metis (no_types) cp_step_is_cdcl\<^sub>W_cp tranclp_into_rtranclp) }
+  then show ?case
+    by fastforce
+next
+  show "no_step cdcl\<^sub>W_cp (toS (rough_state_of (do_full1_cp_step S)))"
+    apply (rule do_cp_step_eq_no_step[OF do_full1_cp_step_fix_point_of_do_full1_cp_step[of S]])
+    using in_clauses_rough_state_of_is_distinct unfolding do_cp_step'_def by blast
+qed
+
+lemma [code abstract]:
+ "rough_state_of (do_cp_step' S) = do_cp_step (rough_state_of S)"
+ unfolding do_cp_step'_def by auto
+
+paragraph \<open>The other rules\<close>
+fun do_other_step where
+"do_other_step S =
+   (let T = do_skip_step S in
+     if T \<noteq> S
+     then T
+     else
+       (let U = do_resolve_step T in
+       if U \<noteq> T
+       then U else
+       (let V = do_backtrack_step U in
+       if V \<noteq> U then V else do_decide_step V)))"
+
+lemma do_other_step:
+  assumes inv: "cdcl\<^sub>W_all_struct_inv (toS S)" and
+  st: "do_other_step S \<noteq> S"
+  shows "cdcl\<^sub>W_o (toS S) (toS (do_other_step S))"
+  using st inv by (auto split: if_split_asm
+    simp add: Let_def
+    intro: do_skip_step do_resolve_step do_backtrack_step do_decide_step)
+
+lemma do_other_step_no:
+  assumes inv: "cdcl\<^sub>W_all_struct_inv (toS S)" and
+  st: "do_other_step S = S"
+  shows "no_step cdcl\<^sub>W_o (toS S)"
+  using st inv by (auto split: if_split_asm elim: cdcl\<^sub>W_bjE
+    simp add: Let_def cdcl\<^sub>W_bj.simps elim!: cdcl\<^sub>W_o.cases
+    dest!: do_skip_step_no do_resolve_step_no do_backtrack_step_no do_decide_step_no)
+
+lemma rough_state_of_state_of_do_other_step[simp]:
+  "rough_state_of (state_of (do_other_step (rough_state_of S))) = do_other_step (rough_state_of S)"
+proof (cases "do_other_step (rough_state_of S) = rough_state_of S")
+  case True
+  then show ?thesis by simp
+next
+  case False
+  have "cdcl\<^sub>W_o (toS (rough_state_of S)) (toS (do_other_step (rough_state_of S)))"
+    by (metis False cdcl\<^sub>W_all_struct_inv_rough_state do_other_step["of" "rough_state_of S"])
+  then have "cdcl\<^sub>W_all_struct_inv (toS (do_other_step (rough_state_of S)))"
+    using cdcl\<^sub>W_all_struct_inv_inv cdcl\<^sub>W_all_struct_inv_rough_state other by blast
+  then show ?thesis
+    by (simp add: CollectI state_of_inverse)
+qed
+
+definition do_other_step' where
+"do_other_step' S =
+  state_of (do_other_step (rough_state_of S))"
+
+lemma rough_state_of_do_other_step'[code abstract]:
+ "rough_state_of (do_other_step' S) = do_other_step (rough_state_of S)"
+ apply (cases "do_other_step (rough_state_of S) = rough_state_of S")
+   unfolding do_other_step'_def apply simp
+ using do_other_step[of "rough_state_of S"] by (auto intro: cdcl\<^sub>W_all_struct_inv_inv
+   cdcl\<^sub>W_all_struct_inv_rough_state other state_of_inverse)
+
+definition do_cdcl\<^sub>W_stgy_step where
+"do_cdcl\<^sub>W_stgy_step S =
+   (let T = do_full1_cp_step S in
+     if T \<noteq> S
+     then T
+     else
+       (let U = (do_other_step' T) in
+        (do_full1_cp_step U))) "
+
+definition do_cdcl\<^sub>W_stgy_step' where
+"do_cdcl\<^sub>W_stgy_step' S = state_from_init_state_of (rough_state_of (do_cdcl\<^sub>W_stgy_step (id_of_I_to S)))"
+
+lemma toS_do_full1_cp_step_not_eq: "do_full1_cp_step S \<noteq> S \<Longrightarrow>
+    toS (rough_state_of S) \<noteq> toS (rough_state_of (do_full1_cp_step S))"
+proof -
+  assume a1: "do_full1_cp_step S \<noteq> S"
+  then have "S \<noteq> do_cp_step' S"
+    by fastforce
+  then show ?thesis
+    by (metis (no_types) cp_step_is_cdcl\<^sub>W_cp do_cp_step'_def do_cp_step_eq_no_step
+      do_full1_cp_step_fix_point_of_do_full1_cp_step in_clauses_rough_state_of_is_distinct
+      rough_state_of_inverse)
+qed
+
+text \<open>@{term do_full1_cp_step} should not be unfolded anymore:\<close>
+declare do_full1_cp_step.simps[simp del]
+
+paragraph \<open>Correction of the transformation\<close>
+lemma do_cdcl\<^sub>W_stgy_step:
+  assumes "do_cdcl\<^sub>W_stgy_step S \<noteq> S"
+  shows "cdcl\<^sub>W_stgy (toS (rough_state_of S)) (toS (rough_state_of (do_cdcl\<^sub>W_stgy_step S)))"
+proof (cases "do_full1_cp_step S = S")
+  case False
+  then show ?thesis
+    using assms do_full1_cp_step_full[of S] unfolding full_unfold do_cdcl\<^sub>W_stgy_step_def
+    by (auto intro!: cdcl\<^sub>W_stgy.intros dest: toS_do_full1_cp_step_not_eq)
+next
+  case True
+  have "cdcl\<^sub>W_o (toS (rough_state_of S)) (toS (rough_state_of (do_other_step' S)))"
+    by (smt True assms cdcl\<^sub>W_all_struct_inv_rough_state do_cdcl\<^sub>W_stgy_step_def do_other_step
+      rough_state_of_do_other_step' rough_state_of_inverse)
+  moreover
+    have
+      np: "no_step propagate (toS (rough_state_of S))" and
+      nc: "no_step conflict (toS (rough_state_of S))"
+        apply (metis True do_cp_step_eq_no_prop_no_confl
+          do_full1_cp_step_fix_point_of_do_full1_cp_step do_propagate_step_no_step
+          in_clauses_rough_state_of_is_distinct)
+      by (metis True do_conflict_step_no_step do_cp_step_eq_no_prop_no_confl
+        do_full1_cp_step_fix_point_of_do_full1_cp_step)
+    then have "no_step cdcl\<^sub>W_cp (toS (rough_state_of S))"
+      by (simp add: cdcl\<^sub>W_cp.simps)
+  moreover have "full cdcl\<^sub>W_cp (toS (rough_state_of (do_other_step' S)))
+    (toS (rough_state_of (do_full1_cp_step (do_other_step' S))))"
+    using do_full1_cp_step_full by auto
+  ultimately show ?thesis
+    using assms True unfolding do_cdcl\<^sub>W_stgy_step_def
+    by (auto intro!: cdcl\<^sub>W_stgy.other' dest: toS_do_full1_cp_step_not_eq)
+qed
+
+lemma length_trail_toS[simp]:
+  "length (trail (toS S)) = length (trail S)"
+  by (cases S) auto
+
+lemma conflicting_noTrue_iff_toS[simp]:
+  "conflicting (toS S) \<noteq> None \<longleftrightarrow> conflicting S \<noteq> None"
+  by (cases S) auto
+
+lemma trail_toS_neq_imp_trail_neq:
+  "trail (toS S) \<noteq> trail (toS S') \<Longrightarrow> trail S \<noteq> trail S'"
+  by (cases S, cases S') auto
+
+lemma do_skip_step_trail_changed_or_conflict:
+  assumes d: "do_other_step S \<noteq> S"
+  and inv: "cdcl\<^sub>W_all_struct_inv (toS S)"
+  shows "trail S \<noteq> trail (do_other_step S)"
+proof -
+  have M: "\<And>M K M1 c. M = c @ K # M1 \<Longrightarrow> Suc (length M1) \<le> length M"
+    by auto
+  have "cdcl\<^sub>W_M_level_inv (toS S)"
+    using inv unfolding cdcl\<^sub>W_all_struct_inv_def by auto
+  have "cdcl\<^sub>W_o (toS S) (toS (do_other_step S))" using do_other_step[OF inv d] .
+  then show ?thesis
+    using \<open>cdcl\<^sub>W_M_level_inv (toS S)\<close>
+    proof (induction "toS (do_other_step S)" rule: cdcl\<^sub>W_o_induct_lev2)
+      case decide
+      then show ?thesis
+        by (auto simp add: trail_toS_neq_imp_trail_neq)[]
+    next
+    case (skip)
+    then show ?case
+      by (cases S; cases "do_other_step S") force
+    next
+      case (resolve)
+      then show ?case
+         by (cases S, cases "do_other_step S") force
+    next
+      case (backtrack K i M1 M2 L D) note decomp = this(1) and confl_S = this(3) and undef = this(6)
+        and U = this(7)
+      have [simp]: "cons_trail (Propagated L (D + {#L#}))
+        (reduce_trail_to M1
+          (add_learned_cls (D + {#L#})
+            (update_backtrack_lvl (get_maximum_level (trail (toS S)) D)
+              (update_conflicting None (toS S)))))
+        =
+        (Propagated L (D + {#L#})# M1,mset (map mset (clss S)),
+          {#D + {#L#}#} + mset (map mset (learned_clss S)),
+          get_maximum_level (trail (toS S)) D, None)"
+        apply (subst state_conv[of "cons_trail _ _"])
+        using decomp undef by (cases S) auto
+      then show ?case
+        apply (cases "do_other_step S")
+        apply (auto split: if_split_asm simp: Let_def)
+            apply (cases S rule: do_skip_step.cases; auto split: if_split_asm)
+           apply (cases S rule: do_skip_step.cases; auto split: if_split_asm)
+
+          apply (cases S rule: do_backtrack_step.cases;
+            auto split: if_split_asm option.splits list.splits marked_lit.splits
+              dest!: bt_cut_some_decomp simp: Let_def)
+        using d apply (cases S rule: do_decide_step.cases; auto split: option.splits)[]
+        done
+    qed
+qed
+
+lemma do_full1_cp_step_induct:
+  "(\<And>S. (S \<noteq>  do_cp_step' S \<Longrightarrow> P (do_cp_step' S)) \<Longrightarrow> P S) \<Longrightarrow> P a0"
+  using do_full1_cp_step.induct by metis
+
+lemma do_cp_step_neq_trail_increase:
+  "\<exists>c. trail (do_cp_step S) = c @ trail  S \<and>(\<forall>m \<in> set c. \<not> is_marked m)"
+  by (cases S, cases "conflicting S")
+     (auto simp add: do_cp_step_def do_conflict_step_def do_propagate_step_def split: option.splits)
+
+lemma do_full1_cp_step_neq_trail_increase:
+  "\<exists>c. trail (rough_state_of (do_full1_cp_step S)) = c @ trail (rough_state_of S)
+    \<and> (\<forall>m \<in> set c. \<not> is_marked m)"
+  apply (induction rule: do_full1_cp_step_induct)
+  apply (rename_tac S, case_tac "do_cp_step' S = S")
+    apply (simp add: do_full1_cp_step.simps)
+  by (smt Un_iff append_assoc do_cp_step'_def do_cp_step_neq_trail_increase do_full1_cp_step.simps
+    rough_state_of_state_of_do_cp_step set_append)
+
+lemma do_cp_step_conflicting:
+  "conflicting (rough_state_of S) \<noteq> None \<Longrightarrow> do_cp_step' S = S"
+  unfolding do_cp_step'_def do_cp_step_def by simp
+
+lemma do_full1_cp_step_conflicting:
+  "conflicting (rough_state_of S) \<noteq> None \<Longrightarrow> do_full1_cp_step S = S"
+  unfolding do_cp_step'_def do_cp_step_def
+  apply (induction rule: do_full1_cp_step_induct)
+  by (rename_tac S, case_tac "S \<noteq> do_cp_step' S")
+   (auto simp add: do_full1_cp_step.simps do_cp_step_conflicting)
+
+lemma do_decide_step_not_conflicting_one_more_decide:
+  assumes
+    "conflicting S = None" and
+    "do_decide_step S \<noteq> S"
+  shows "Suc (length (filter is_marked (trail S)))
+    = length (filter is_marked (trail (do_decide_step S)))"
+  using assms unfolding do_other_step'_def
+  by (cases S) (auto simp: Let_def split: if_split_asm option.splits
+     dest!: find_first_unused_var_Some_not_all_incl)
+
+lemma do_decide_step_not_conflicting_one_more_decide_bt:
+  assumes "conflicting S \<noteq> None" and
+  "do_decide_step S \<noteq> S"
+  shows "length (filter is_marked (trail S)) < length (filter is_marked (trail (do_decide_step S)))"
+  using assms unfolding do_other_step'_def by (cases S, cases "conflicting S")
+    (auto simp add: Let_def split: if_split_asm option.splits)
+
+lemma do_other_step_not_conflicting_one_more_decide_bt:
+  assumes
+    "conflicting (rough_state_of S) \<noteq> None" and
+    "conflicting (rough_state_of (do_other_step' S)) = None" and
+    "do_other_step' S \<noteq> S"
+  shows "length (filter is_marked (trail (rough_state_of S)))
+    > length (filter is_marked (trail (rough_state_of (do_other_step' S))))"
+proof (cases S, goal_cases)
+  case (1 y) note S = this(1) and inv = this(2)
+  obtain M N U k E where y: "y = (M, N, U, k, Some E)"
+    using assms(1) S inv by (cases y, cases "conflicting y") auto
+  have M: "rough_state_of (state_of (M, N, U, k,  Some E)) = (M, N, U, k,  Some E)"
+    using inv y by (auto simp add: state_of_inverse)
+  have bt: "do_other_step' S = state_of (do_backtrack_step (rough_state_of S))"
+    proof (cases "rough_state_of S" rule: do_decide_step.cases)
+      case 1
+      then show ?thesis
+        using assms(1,2) by auto[]
+    next
+      case (2 v vb vd vf vh)
+      have f3: "\<And>c. (if do_skip_step (rough_state_of c) \<noteq> rough_state_of c
+        then do_skip_step (rough_state_of c)
+        else if do_resolve_step (do_skip_step (rough_state_of c)) \<noteq> do_skip_step (rough_state_of c)
+             then do_resolve_step (do_skip_step (rough_state_of c))
+             else if do_backtrack_step (do_resolve_step (do_skip_step (rough_state_of c)))
+               \<noteq> do_resolve_step (do_skip_step (rough_state_of c))
+             then do_backtrack_step (do_resolve_step (do_skip_step (rough_state_of c)))
+             else do_decide_step (do_backtrack_step (do_resolve_step
+               (do_skip_step (rough_state_of c)))))
+        = rough_state_of (do_other_step' c)"
+        by (simp add: rough_state_of_do_other_step')
+      have "(trail (rough_state_of (do_other_step' S)), clss (rough_state_of (do_other_step' S)),
+          learned_clss (rough_state_of (do_other_step' S)),
+          backtrack_lvl (rough_state_of (do_other_step' S)), None)
+        = rough_state_of (do_other_step' S)"
+        using assms(2) by (metis (no_types) state_conv)
+      then show ?thesis
+        using f3 2 by (metis (no_types) do_decide_step.simps(2) do_resolve_step_trail_is_None
+          do_skip_step_trail_is_None rough_state_of_inverse)
+    qed
+  show ?case
+    using assms(2) S unfolding bt y inv
+    apply simp
+    by (auto simp add: M bt_cut_not_none
+          split: option.splits
+          dest!: bt_cut_some_decomp)
+qed
+
+lemma do_other_step_not_conflicting_one_more_decide:
+  assumes "conflicting (rough_state_of S) = None" and
+  "do_other_step' S \<noteq> S"
+  shows "1 + length (filter is_marked (trail (rough_state_of S)))
+    = length (filter is_marked (trail (rough_state_of (do_other_step' S))))"
+proof (cases S, goal_cases)
+  case (1 y) note S = this(1) and inv = this(2)
+  obtain M N U k where y: "y = (M, N, U, k, None)" using assms(1) S inv by (cases y) auto
+  have M: "rough_state_of (state_of (M, N, U, k, None)) = (M, N, U, k, None)"
+    using inv y by (auto simp add: state_of_inverse)
+  have "state_of (do_decide_step (M, N, U, k, None)) \<noteq> state_of (M, N, U, k, None)"
+    using assms(2) unfolding do_other_step'_def y inv S by (auto simp add: M)
+  then have f4: "do_skip_step (rough_state_of S) = rough_state_of S"
+    unfolding S M y by (metis (full_types) do_skip_step.simps(4))
+  have f5: "do_resolve_step (rough_state_of S) = rough_state_of S"
+    unfolding S M y by (metis (no_types) do_resolve_step.simps(4))
+  have f6: "do_backtrack_step (rough_state_of S) = rough_state_of S"
+    unfolding S M y by (metis (no_types) do_backtrack_step.simps(2))
+  have "do_other_step (rough_state_of S) \<noteq> rough_state_of S"
+    using assms(2) unfolding S M y do_other_step'_def by (metis (no_types))
+  then show ?case
+    using f6 f5 f4 by (simp add: assms(1) do_decide_step_not_conflicting_one_more_decide
+      do_other_step'_def)
+qed
+
+lemma rough_state_of_state_of_do_skip_step_rough_state_of[simp]:
+  "rough_state_of (state_of (do_skip_step (rough_state_of S))) = do_skip_step (rough_state_of S)"
+  by (smt do_other_step.simps rough_state_of_inverse rough_state_of_state_of_do_other_step)
+
+lemma conflicting_do_resolve_step_iff[iff]:
+  "conflicting (do_resolve_step S) = None \<longleftrightarrow> conflicting S = None"
+  by (cases S rule: do_resolve_step.cases)
+   (auto simp add: Let_def split: option.splits)
+
+lemma conflicting_do_skip_step_iff[iff]:
+  "conflicting (do_skip_step S) = None \<longleftrightarrow> conflicting S = None"
+  by (cases S rule: do_skip_step.cases)
+     (auto simp add: Let_def split: option.splits)
+
+lemma conflicting_do_decide_step_iff[iff]:
+  "conflicting (do_decide_step S) = None \<longleftrightarrow> conflicting S = None"
+  by (cases S rule: do_decide_step.cases)
+     (auto simp add: Let_def split: option.splits)
+
+lemma conflicting_do_backtrack_step_imp[simp]:
+  "do_backtrack_step S \<noteq> S \<Longrightarrow> conflicting (do_backtrack_step S) = None"
+  by (cases S rule: do_backtrack_step.cases)
+     (auto simp add: Let_def split: list.splits option.splits marked_lit.splits)
+
+lemma do_skip_step_eq_iff_trail_eq:
+  "do_skip_step S = S \<longleftrightarrow> trail (do_skip_step S) = trail S"
+  by (cases S rule: do_skip_step.cases) auto
+
+lemma do_decide_step_eq_iff_trail_eq:
+  "do_decide_step S = S \<longleftrightarrow> trail (do_decide_step S) = trail S"
+  by (cases S rule: do_decide_step.cases) (auto split: option.split)
+
+lemma do_backtrack_step_eq_iff_trail_eq:
+  "do_backtrack_step S = S \<longleftrightarrow> trail (do_backtrack_step S) = trail S"
+  by (cases S rule: do_backtrack_step.cases)
+     (auto split: option.split list.splits marked_lit.splits
+       dest!: bt_cut_in_get_all_marked_decomposition)
+
+lemma do_resolve_step_eq_iff_trail_eq:
+  "do_resolve_step S = S \<longleftrightarrow> trail (do_resolve_step S) = trail S"
+  by (cases S rule: do_resolve_step.cases) auto
+
+lemma do_other_step_eq_iff_trail_eq:
+  "trail (do_other_step S) = trail S \<longleftrightarrow> do_other_step S = S"
+  by (auto simp add: Let_def do_skip_step_eq_iff_trail_eq[symmetric]
+    do_decide_step_eq_iff_trail_eq[symmetric] do_backtrack_step_eq_iff_trail_eq[symmetric]
+    do_resolve_step_eq_iff_trail_eq[symmetric])
+
+
+lemma do_full1_cp_step_do_other_step'_normal_form[dest!]:
+  assumes H: "do_full1_cp_step (do_other_step' S) = S"
+  shows "do_other_step' S = S \<and> do_full1_cp_step S = S"
+proof -
+  let ?T = "do_other_step' S"
+  { assume confl: "conflicting (rough_state_of ?T) \<noteq> None"
+    then have tr: "trail (rough_state_of (do_full1_cp_step ?T)) = trail (rough_state_of ?T)"
+      using do_full1_cp_step_conflicting by auto
+    have "trail (rough_state_of (do_full1_cp_step (do_other_step' S))) = trail (rough_state_of S)"
+      using arg_cong[OF H, of "\<lambda>S. trail (rough_state_of S)"] .
+    then have "trail (rough_state_of (do_other_step' S)) = trail (rough_state_of S)"
+       by (auto simp add: do_full1_cp_step_conflicting confl)
+    then have "do_other_step' S = S"
+      by (simp add: do_other_step_eq_iff_trail_eq do_other_step'_def
+        del: do_other_step.simps)
+  }
+  moreover {
+    assume eq[simp]: "do_other_step' S = S"
+    obtain c where c: "trail (rough_state_of (do_full1_cp_step S)) = c @ trail (rough_state_of S)"
+      using do_full1_cp_step_neq_trail_increase by auto
+
+    moreover have "trail (rough_state_of (do_full1_cp_step S)) = trail (rough_state_of S)"
+      using arg_cong[OF H, of "\<lambda>S. trail (rough_state_of S)"] by simp
+    finally have "c = []" by blast
+    then have "do_full1_cp_step S = S" using assms by auto
+    }
+  moreover {
+    assume confl: "conflicting (rough_state_of ?T) = None" and neq: "do_other_step' S \<noteq> S"
+    obtain c where
+      c: "trail (rough_state_of (do_full1_cp_step ?T)) = c @ trail (rough_state_of ?T)" and
+      nm: "\<forall>m\<in>set c. \<not> is_marked m"
+      using do_full1_cp_step_neq_trail_increase by auto
+    have "length (filter is_marked (trail (rough_state_of (do_full1_cp_step ?T))))
+       = length (filter is_marked (trail (rough_state_of ?T)))" using nm unfolding c by force
+    moreover have "length (filter is_marked (trail (rough_state_of S)))
+       \<noteq> length (filter is_marked  (trail (rough_state_of ?T)))"
+      using do_other_step_not_conflicting_one_more_decide[OF _ neq]
+      do_other_step_not_conflicting_one_more_decide_bt[of S, OF _ confl neq]
+      by linarith
+    finally have False unfolding H by blast
+  }
+  ultimately show ?thesis by blast
+qed
+
+lemma do_cdcl\<^sub>W_stgy_step_no:
+  assumes S: "do_cdcl\<^sub>W_stgy_step S = S"
+  shows "no_step cdcl\<^sub>W_stgy (toS (rough_state_of S))"
+proof -
+  {
+    fix S'
+    assume "full1 cdcl\<^sub>W_cp (toS (rough_state_of S)) S'"
+    then have False
+      using do_full1_cp_step_full[of S] unfolding full_def S rtranclp_unfold full1_def
+      by (smt assms do_cdcl\<^sub>W_stgy_step_def tranclpD)
+  }
+  moreover {
+    fix S' S''
+    assume " cdcl\<^sub>W_o (toS (rough_state_of S)) S'" and
+     "no_step propagate (toS (rough_state_of S))" and
+     "no_step conflict (toS (rough_state_of S))" and
+     "full cdcl\<^sub>W_cp S' S''"
+    then have False
+      using assms unfolding do_cdcl\<^sub>W_stgy_step_def
+      by (smt cdcl\<^sub>W_all_struct_inv_rough_state do_full1_cp_step_do_other_step'_normal_form
+        do_other_step_no rough_state_of_do_other_step')
+  }
+  ultimately show ?thesis using assms by (force simp: cdcl\<^sub>W_cp.simps cdcl\<^sub>W_stgy.simps)
+qed
+
+lemma toS_rough_state_of_state_of_rough_state_from_init_state_of[simp]:
+  "toS (rough_state_of (state_of (rough_state_from_init_state_of S)))
+    = toS (rough_state_from_init_state_of S)"
+  using rough_state_from_init_state_of[of S] by (auto simp add: state_of_inverse)
+
+lemma cdcl\<^sub>W_cp_is_rtranclp_cdcl\<^sub>W: "cdcl\<^sub>W_cp S T \<Longrightarrow> cdcl\<^sub>W\<^sup>*\<^sup>* S T"
+  apply (induction rule: cdcl\<^sub>W_cp.induct)
+   using conflict apply blast
+  using propagate by blast
+
+lemma rtranclp_cdcl\<^sub>W_cp_is_rtranclp_cdcl\<^sub>W: "cdcl\<^sub>W_cp\<^sup>*\<^sup>* S T \<Longrightarrow> cdcl\<^sub>W\<^sup>*\<^sup>* S T"
+  apply (induction rule: rtranclp_induct)
+    apply simp
+  by (fastforce dest!: cdcl\<^sub>W_cp_is_rtranclp_cdcl\<^sub>W)
+
+lemma cdcl\<^sub>W_stgy_is_rtranclp_cdcl\<^sub>W:
+  "cdcl\<^sub>W_stgy S T \<Longrightarrow> cdcl\<^sub>W\<^sup>*\<^sup>* S T"
+  apply (induction rule: cdcl\<^sub>W_stgy.induct)
+   using cdcl\<^sub>W_stgy.conflict' rtranclp_cdcl\<^sub>W_stgy_rtranclp_cdcl\<^sub>W apply blast
+  unfolding full_def by (fastforce dest!:other rtranclp_cdcl\<^sub>W_cp_is_rtranclp_cdcl\<^sub>W)
+
+lemma cdcl\<^sub>W_stgy_init_clss: "cdcl\<^sub>W_stgy S T \<Longrightarrow> cdcl\<^sub>W_M_level_inv S \<Longrightarrow> clss S = clss T"
+  using rtranclp_cdcl\<^sub>W_init_clss cdcl\<^sub>W_stgy_is_rtranclp_cdcl\<^sub>W by fast
+
+lemma clauses_toS_rough_state_of_do_cdcl\<^sub>W_stgy_step[simp]:
+  "clss (toS (rough_state_of (do_cdcl\<^sub>W_stgy_step (state_of (rough_state_from_init_state_of S)))))
+    = clss (toS (rough_state_from_init_state_of S))" (is "_ = clss (toS ?S)")
+  apply (cases "do_cdcl\<^sub>W_stgy_step (state_of ?S) = state_of ?S")
+    apply simp
+  by (smt cdcl\<^sub>W_all_struct_inv_def cdcl\<^sub>W_all_struct_inv_rough_state cdcl\<^sub>W_stgy_no_more_init_clss
+    do_cdcl\<^sub>W_stgy_step toS_rough_state_of_state_of_rough_state_from_init_state_of)
+
+lemma rough_state_from_init_state_of_do_cdcl\<^sub>W_stgy_step'[code abstract]:
+ "rough_state_from_init_state_of (do_cdcl\<^sub>W_stgy_step' S) =
+   rough_state_of (do_cdcl\<^sub>W_stgy_step (id_of_I_to S))"
+proof -
+  let ?S = "(rough_state_from_init_state_of S)"
+  have "cdcl\<^sub>W_stgy\<^sup>*\<^sup>* (S0_cdcl\<^sub>W (clss (toS (rough_state_from_init_state_of S))))
+    (toS (rough_state_from_init_state_of S))"
+    using rough_state_from_init_state_of[of S] by auto
+  moreover have "cdcl\<^sub>W_stgy\<^sup>*\<^sup>*
+                  (toS (rough_state_from_init_state_of S))
+                  (toS (rough_state_of (do_cdcl\<^sub>W_stgy_step
+                    (state_of (rough_state_from_init_state_of S)))))"
+     using do_cdcl\<^sub>W_stgy_step[of "state_of ?S"]
+     by (cases "do_cdcl\<^sub>W_stgy_step (state_of ?S) = state_of ?S") auto
+  ultimately show ?thesis
+    unfolding do_cdcl\<^sub>W_stgy_step'_def id_of_I_to_def
+    by (auto intro!: state_from_init_state_of_inverse)
+qed
+
+paragraph \<open>All rules together\<close>
+function do_all_cdcl\<^sub>W_stgy where
+"do_all_cdcl\<^sub>W_stgy S =
+  (let T = do_cdcl\<^sub>W_stgy_step' S in
+  if T = S then S else do_all_cdcl\<^sub>W_stgy T)"
+by fast+
+termination
+proof (relation "{(T, S).
+    (cdcl\<^sub>W_measure (toS (rough_state_from_init_state_of T)),
+    cdcl\<^sub>W_measure (toS (rough_state_from_init_state_of S)))
+      \<in> lexn {(a, b). a < b} 3}", goal_cases)
+  case 1
+  show ?case by (rule wf_if_measure_f) (auto intro!: wf_lexn wf_less)
+next
+  case (2 S T) note T = this(1) and ST = this(2)
+  let ?S = "rough_state_from_init_state_of S"
+  have S: "cdcl\<^sub>W_stgy\<^sup>*\<^sup>* (S0_cdcl\<^sub>W (clss (toS ?S))) (toS ?S)"
+    using rough_state_from_init_state_of[of S] by auto
+  moreover have "cdcl\<^sub>W_stgy (toS (rough_state_from_init_state_of S))
+    (toS (rough_state_from_init_state_of T))"
+    proof -
+      have "\<And>c. rough_state_of (state_of (rough_state_from_init_state_of c)) =
+        rough_state_from_init_state_of c"
+        using rough_state_from_init_state_of by force
+      then have "do_cdcl\<^sub>W_stgy_step (state_of (rough_state_from_init_state_of S))
+        \<noteq> state_of (rough_state_from_init_state_of S)"
+        using ST T by (metis (no_types) id_of_I_to_def rough_state_from_init_state_of_inject
+          rough_state_from_init_state_of_do_cdcl\<^sub>W_stgy_step')
+      then show ?thesis
+        using do_cdcl\<^sub>W_stgy_step id_of_I_to_def rough_state_from_init_state_of_do_cdcl\<^sub>W_stgy_step' T
+        by fastforce
+    qed
+  moreover
+    have "cdcl\<^sub>W_all_struct_inv (toS (rough_state_from_init_state_of S))"
+      using rough_state_from_init_state_of[of S] by auto
+    then have "cdcl\<^sub>W_all_struct_inv (S0_cdcl\<^sub>W (clss (toS (rough_state_from_init_state_of S))))"
+      by (cases "rough_state_from_init_state_of S")
+         (auto simp add: cdcl\<^sub>W_all_struct_inv_def distinct_cdcl\<^sub>W_state_def)
+  ultimately show ?case
+    by (auto intro!: cdcl\<^sub>W_stgy_step_decreasing[of _ _ "S0_cdcl\<^sub>W (clss (toS ?S))"]
+      simp del: cdcl\<^sub>W_measure.simps)
+qed
+
+thm do_all_cdcl\<^sub>W_stgy.induct
+lemma do_all_cdcl\<^sub>W_stgy_induct:
+  "(\<And>S. (do_cdcl\<^sub>W_stgy_step' S \<noteq> S \<Longrightarrow> P (do_cdcl\<^sub>W_stgy_step' S)) \<Longrightarrow> P S) \<Longrightarrow> P a0"
+ using do_all_cdcl\<^sub>W_stgy.induct by metis
+
+lemma no_step_cdcl\<^sub>W_stgy_cdcl\<^sub>W_all:
+  "no_step cdcl\<^sub>W_stgy (toS (rough_state_from_init_state_of (do_all_cdcl\<^sub>W_stgy S)))"
+  apply (induction S rule:do_all_cdcl\<^sub>W_stgy_induct)
+  apply (rename_tac S, case_tac "do_cdcl\<^sub>W_stgy_step' S \<noteq> S")
+proof -
+  fix Sa :: cdcl\<^sub>W_state_inv_from_init_state
+  assume a1: "\<not> do_cdcl\<^sub>W_stgy_step' Sa \<noteq> Sa"
+  { fix pp
+    have "(if True then Sa else do_all_cdcl\<^sub>W_stgy Sa) = do_all_cdcl\<^sub>W_stgy Sa"
+      using a1 by auto
+    then have "\<not> cdcl\<^sub>W_stgy (toS (rough_state_from_init_state_of (do_all_cdcl\<^sub>W_stgy Sa))) pp"
+      using a1 by (metis (no_types) do_cdcl\<^sub>W_stgy_step_no id_of_I_to_def
+        rough_state_from_init_state_of_do_cdcl\<^sub>W_stgy_step' rough_state_of_inverse) }
+  then show "no_step cdcl\<^sub>W_stgy (toS (rough_state_from_init_state_of (do_all_cdcl\<^sub>W_stgy Sa)))"
+    by fastforce
+next
+  fix Sa :: cdcl\<^sub>W_state_inv_from_init_state
+  assume a1: "do_cdcl\<^sub>W_stgy_step' Sa \<noteq> Sa
+    \<Longrightarrow> no_step cdcl\<^sub>W_stgy (toS (rough_state_from_init_state_of
+      (do_all_cdcl\<^sub>W_stgy (do_cdcl\<^sub>W_stgy_step' Sa))))"
+  assume a2: "do_cdcl\<^sub>W_stgy_step' Sa \<noteq> Sa"
+  have "do_all_cdcl\<^sub>W_stgy Sa = do_all_cdcl\<^sub>W_stgy (do_cdcl\<^sub>W_stgy_step' Sa)"
+    by (metis (full_types) do_all_cdcl\<^sub>W_stgy.simps)
+  then show "no_step cdcl\<^sub>W_stgy (toS (rough_state_from_init_state_of (do_all_cdcl\<^sub>W_stgy Sa)))"
+    using a2 a1 by presburger
+qed
+
+lemma do_all_cdcl\<^sub>W_stgy_is_rtranclp_cdcl\<^sub>W_stgy:
+  "cdcl\<^sub>W_stgy\<^sup>*\<^sup>* (toS (rough_state_from_init_state_of S))
+    (toS (rough_state_from_init_state_of (do_all_cdcl\<^sub>W_stgy S)))"
+proof (induction S rule: do_all_cdcl\<^sub>W_stgy_induct)
+  case (1 S) note IH = this(1)
+  show ?case
+    proof (cases "do_cdcl\<^sub>W_stgy_step' S = S")
+      case True
+      then show ?thesis by simp
+    next
+      case False
+      have f2: "do_cdcl\<^sub>W_stgy_step (id_of_I_to S) = id_of_I_to S \<longrightarrow>
+        rough_state_from_init_state_of (do_cdcl\<^sub>W_stgy_step' S)
+        = rough_state_of (state_of (rough_state_from_init_state_of S))"
+        using id_of_I_to_def rough_state_from_init_state_of_do_cdcl\<^sub>W_stgy_step' by presburger
+      have f3: "do_all_cdcl\<^sub>W_stgy S = do_all_cdcl\<^sub>W_stgy (do_cdcl\<^sub>W_stgy_step' S)"
+        by (metis (full_types) do_all_cdcl\<^sub>W_stgy.simps)
+      have "cdcl\<^sub>W_stgy (toS (rough_state_from_init_state_of S))
+          (toS (rough_state_from_init_state_of (do_cdcl\<^sub>W_stgy_step' S)))
+        = cdcl\<^sub>W_stgy (toS (rough_state_of (id_of_I_to S)))
+          (toS (rough_state_of (do_cdcl\<^sub>W_stgy_step (id_of_I_to S))))"
+        using id_of_I_to_def rough_state_from_init_state_of_do_cdcl\<^sub>W_stgy_step'
+        toS_rough_state_of_state_of_rough_state_from_init_state_of by presburger
+      then show ?thesis
+        using f3 f2 IH do_cdcl\<^sub>W_stgy_step by fastforce
+    qed
+qed
+
+text \<open>Final theorem:\<close>
+lemma DPLL_tot_correct:
+  assumes
+    r: "rough_state_from_init_state_of (do_all_cdcl\<^sub>W_stgy (state_from_init_state_of
+      (([], map remdups N, [], 0, None)))) = S" and
+    S: "(M', N', U', k, E) = toS S"
+  shows "(E \<noteq> Some {#} \<and> satisfiable (set (map mset N)))
+    \<or> (E = Some {#} \<and> unsatisfiable (set (map mset N)))"
+proof -
+  let ?N = "map remdups N"
+  have inv: "cdcl\<^sub>W_all_struct_inv (toS ([], map remdups N, [], 0, None))"
+    unfolding cdcl\<^sub>W_all_struct_inv_def distinct_cdcl\<^sub>W_state_def distinct_mset_set_def by auto
+  then have S0: "rough_state_of (state_of ([], map remdups N, [], 0, None))
+    = ([], map remdups N, [], 0, None)" by simp
+  have 1: "full cdcl\<^sub>W_stgy (toS ([], ?N, [], 0, None)) (toS S)"
+    unfolding full_def apply rule
+      using do_all_cdcl\<^sub>W_stgy_is_rtranclp_cdcl\<^sub>W_stgy[of
+        "state_from_init_state_of ([], map remdups N, [], 0, None)"] inv
+        no_step_cdcl\<^sub>W_stgy_cdcl\<^sub>W_all
+        by (auto simp del: do_all_cdcl\<^sub>W_stgy.simps simp: state_from_init_state_of_inverse
+          r[symmetric])+
+  moreover have 2: "finite (set (map mset ?N))" by auto
+  moreover have 3: "distinct_mset_set (set (map mset ?N))"
+     unfolding distinct_mset_set_def by auto
+  moreover
+    have "cdcl\<^sub>W_all_struct_inv (toS S)"
+      by (metis (no_types) cdcl\<^sub>W_all_struct_inv_rough_state r
+        toS_rough_state_of_state_of_rough_state_from_init_state_of)
+    then have cons: "consistent_interp (lits_of M')"
+      unfolding cdcl\<^sub>W_all_struct_inv_def cdcl\<^sub>W_M_level_inv_def S[symmetric] by auto
+  moreover
+    have "clss (toS ([], ?N, [], 0, None)) = clss (toS S)"
+      apply (rule rtranclp_cdcl\<^sub>W_init_clss)
+      using 1 unfolding full_def by (auto simp add: rtranclp_cdcl\<^sub>W_stgy_rtranclp_cdcl\<^sub>W)
+    then have N': "mset (map mset ?N) = N'"
+      using S[symmetric] by auto
+  have "(E \<noteq> Some {#} \<and> satisfiable (set (map mset ?N)))
+    \<or> (E = Some {#} \<and> unsatisfiable (set (map mset ?N)))"
+    using full_cdcl\<^sub>W_stgy_final_state_conclusive unfolding N' apply rule
+        using 1 apply simp
+       using 2 apply simp
+      using 3 apply simp
+     using S[symmetric] N' apply auto[1]
+   using S[symmetric] N' cons by (fastforce simp: true_annots_true_cls)
+  then show ?thesis by auto
+qed
+
+paragraph \<open>The Code\<close>
+text \<open>The SML code is skipped in the documentation, but stays to ensure that some version of the
+ exported code is working. The only difference between the generated code and the one used here is
+ the export of the constructor ConI.\<close>
+(*<*)
+fun gene where
+"gene 0 = [[Pos 0], [Neg 0]]" |
+"gene (Suc n) = map (op # (Pos (Suc n))) (gene n) @ map (op # (Neg (Suc n))) (gene n)"
+
+value "gene 1"
+
+export_code do_all_cdcl\<^sub>W_stgy gene in SML
+ML \<open>
+structure HOL : sig
+  type 'a equal
+  val equal : 'a equal -> 'a -> 'a -> bool
+  val eq : 'a equal -> 'a -> 'a -> bool
+end = struct
+
+type 'a equal = {equal : 'a -> 'a -> bool};
+val equal = #equal : 'a equal -> 'a -> 'a -> bool;
+
+fun eq A_ a b = equal A_ a b;
+
+end; (*struct HOL*)
+
+structure List : sig
+  val equal_list : 'a HOL.equal -> ('a list) HOL.equal
+  val fold : ('a -> 'b -> 'b) -> 'a list -> 'b -> 'b
+  val rev : 'a list -> 'a list
+  val find : ('a -> bool) -> 'a list -> 'a option
+  val null : 'a list -> bool
+  val filter : ('a -> bool) -> 'a list -> 'a list
+  val member : 'a HOL.equal -> 'a list -> 'a -> bool
+  val remdups : 'a HOL.equal -> 'a list -> 'a list
+  val remove1 : 'a HOL.equal -> 'a -> 'a list -> 'a list
+  val map : ('a -> 'b) -> 'a list -> 'b list
+  val list_all : ('a -> bool) -> 'a list -> bool
+end = struct
+
+fun equal_lista A_ [] (x21 :: x22) = false
+  | equal_lista A_ (x21 :: x22) [] = false
+  | equal_lista A_ (x21 :: x22) (y21 :: y22) =
+    HOL.eq A_ x21 y21 andalso equal_lista A_ x22 y22
+  | equal_lista A_ [] [] = true;
+
+fun equal_list A_ = {equal = equal_lista A_} : ('a list) HOL.equal;
+
+fun fold f (x :: xs) s = fold f xs (f x s)
+  | fold f [] s = s;
+
+fun rev xs = fold (fn a => fn b => a :: b) xs [];
+
+fun find uu [] = NONE
+  | find p (x :: xs) = (if p x then SOME x else find p xs);
+
+fun null [] = true
+  | null (x :: xs) = false;
+
+fun filter p [] = []
+  | filter p (x :: xs) = (if p x then x :: filter p xs else filter p xs);
+
+fun member A_ [] y = false
+  | member A_ (x :: xs) y = HOL.eq A_ x y orelse member A_ xs y;
+
+fun remdups A_ [] = []
+  | remdups A_ (x :: xs) =
+    (if member A_ xs x then remdups A_ xs else x :: remdups A_ xs);
+
+fun remove1 A_ x [] = []
+  | remove1 A_ x (y :: xs) =
+    (if HOL.eq A_ x y then xs else y :: remove1 A_ x xs);
+
+fun map f [] = []
+  | map f (x21 :: x22) = f x21 :: map f x22;
+
+fun list_all p [] = true
+  | list_all p (x :: xs) = p x andalso list_all p xs;
+
+end; (*struct List*)
+
+structure Set : sig
+  datatype 'a set = Set of 'a list | Coset of 'a list
+  val image : ('a -> 'b) -> 'a set -> 'b set
+  val member : 'a HOL.equal -> 'a -> 'a set -> bool
+end = struct
+
+datatype 'a set = Set of 'a list | Coset of 'a list;
+
+fun image f (Set xs) = Set (List.map f xs);
+
+fun member A_ x (Coset xs) = not (List.member A_ xs x)
+  | member A_ x (Set xs) = List.member A_ xs x;
+
+end; (*struct Set*)
+
+structure Orderings : sig
+  type 'a ord
+  val less_eq : 'a ord -> 'a -> 'a -> bool
+  val less : 'a ord -> 'a -> 'a -> bool
+  type 'a preorder
+  val ord_preorder : 'a preorder -> 'a ord
+  type 'a order
+  val preorder_order : 'a order -> 'a preorder
+  type 'a linorder
+  val order_linorder : 'a linorder -> 'a order
+  val max : 'a ord -> 'a -> 'a -> 'a
+end = struct
+
+type 'a ord = {less_eq : 'a -> 'a -> bool, less : 'a -> 'a -> bool};
+val less_eq = #less_eq : 'a ord -> 'a -> 'a -> bool;
+val less = #less : 'a ord -> 'a -> 'a -> bool;
+
+type 'a preorder = {ord_preorder : 'a ord};
+val ord_preorder = #ord_preorder : 'a preorder -> 'a ord;
+
+type 'a order = {preorder_order : 'a preorder};
+val preorder_order = #preorder_order : 'a order -> 'a preorder;
+
+type 'a linorder = {order_linorder : 'a order};
+val order_linorder = #order_linorder : 'a linorder -> 'a order;
+
+fun max A_ a b = (if less_eq A_ a b then b else a);
+
+end; (*struct Orderings*)
+
+structure Arith : sig
+  datatype nat = Zero_nat | Suc of nat
+  val equal_nata : nat -> nat -> bool
+  val equal_nat : nat HOL.equal
+  val less_nat : nat -> nat -> bool
+  val linorder_nat : nat Orderings.linorder
+  val one_nat : nat
+  val plus_nat : nat -> nat -> nat
+end = struct
+
+datatype nat = Zero_nat | Suc of nat;
+
+fun equal_nata Zero_nat (Suc x2) = false
+  | equal_nata (Suc x2) Zero_nat = false
+  | equal_nata (Suc x2) (Suc y2) = equal_nata x2 y2
+  | equal_nata Zero_nat Zero_nat = true;
+
+val equal_nat = {equal = equal_nata} : nat HOL.equal;
+
+fun less_eq_nat (Suc m) n = less_nat m n
+  | less_eq_nat Zero_nat n = true
+and less_nat m (Suc n) = less_eq_nat m n
+  | less_nat n Zero_nat = false;
+
+val ord_nat = {less_eq = less_eq_nat, less = less_nat} : nat Orderings.ord;
+
+val preorder_nat = {ord_preorder = ord_nat} : nat Orderings.preorder;
+
+val order_nat = {preorder_order = preorder_nat} : nat Orderings.order;
+
+val linorder_nat = {order_linorder = order_nat} : nat Orderings.linorder;
+
+val one_nat : nat = Suc Zero_nat;
+
+fun plus_nat (Suc m) n = plus_nat m (Suc n)
+  | plus_nat Zero_nat n = n;
+
+end; (*struct Arith*)
+
+structure Option : sig
+  val equal_option : 'a HOL.equal -> ('a option) HOL.equal
+end = struct
+
+fun equal_optiona A_ NONE (SOME x2) = false
+  | equal_optiona A_ (SOME x2) NONE = false
+  | equal_optiona A_ (SOME x2) (SOME y2) = HOL.eq A_ x2 y2
+  | equal_optiona A_ NONE NONE = true;
+
+fun equal_option A_ = {equal = equal_optiona A_} : ('a option) HOL.equal;
+
+end; (*struct Option*)
+
+structure Multiset : sig
+  datatype 'a multiset = Mset of 'a list
+  val single : 'a -> 'a multiset
+  val set_mset : 'a multiset -> 'a Set.set
+  val image_mset : ('a -> 'b) -> 'a multiset -> 'b multiset
+  val plus_multiset : 'a multiset -> 'a multiset -> 'a multiset
+end = struct
+
+datatype 'a multiset = Mset of 'a list;
+
+fun single x = Mset [x];
+
+fun set_mset (Mset x) = Set.Set x;
+
+fun image_mset f (Mset xs) = Mset (List.map f xs);
+
+fun plus_multiset (Mset xs) (Mset ys) = Mset (xs @ ys);
+
+end; (*struct Multiset*)
+
+structure Clausal_Logic : sig
+  datatype 'a literal = Pos of 'a | Neg of 'a
+  val equal_literala : 'a HOL.equal -> 'a literal -> 'a literal -> bool
+  val equal_literal : 'a HOL.equal -> 'a literal HOL.equal
+  val atm_of : 'a literal -> 'a
+  val uminus_literal : 'a literal -> 'a literal
+end = struct
+
+datatype 'a literal = Pos of 'a | Neg of 'a;
+
+fun equal_literala A_ (Pos x1) (Neg x2) = false
+  | equal_literala A_ (Neg x2) (Pos x1) = false
+  | equal_literala A_ (Neg x2) (Neg y2) = HOL.eq A_ x2 y2
+  | equal_literala A_ (Pos x1) (Pos y1) = HOL.eq A_ x1 y1;
+
+fun equal_literal A_ = {equal = equal_literala A_} : 'a literal HOL.equal;
+
+fun atm_of (Pos x1) = x1
+  | atm_of (Neg x2) = x2;
+
+fun is_pos (Pos x1) = true
+  | is_pos (Neg x2) = false;
+
+fun uminus_literal l = (if is_pos l then Neg else Pos) (atm_of l);
+
+end; (*struct Clausal_Logic*)
+
+structure Partial_Annotated_Clausal_Logic : sig
+  datatype ('a, 'b, 'c) marked_lit = Marked of 'a Clausal_Logic.literal * 'b |
+    Propagated of 'a Clausal_Logic.literal * 'c
+  val equal_marked_lit :
+    'a HOL.equal -> 'b HOL.equal -> 'c HOL.equal ->
+      ('a, 'b, 'c) marked_lit HOL.equal
+  val lits_of : ('a, 'b, 'c) marked_lit list -> 'a Clausal_Logic.literal Set.set
+end = struct
+
+datatype ('a, 'b, 'c) marked_lit = Marked of 'a Clausal_Logic.literal * 'b |
+  Propagated of 'a Clausal_Logic.literal * 'c;
+
+fun equal_marked_lita A_ B_ C_ (Marked (x11, x12)) (Propagated (x21, x22)) =
+  false
+  | equal_marked_lita A_ B_ C_ (Propagated (x21, x22)) (Marked (x11, x12)) =
+    false
+  | equal_marked_lita A_ B_ C_ (Propagated (x21, x22)) (Propagated (y21, y22)) =
+    Clausal_Logic.equal_literala A_ x21 y21 andalso HOL.eq C_ x22 y22
+  | equal_marked_lita A_ B_ C_ (Marked (x11, x12)) (Marked (y11, y12)) =
+    Clausal_Logic.equal_literala A_ x11 y11 andalso HOL.eq B_ x12 y12;
+
+fun equal_marked_lit A_ B_ C_ = {equal = equal_marked_lita A_ B_ C_} :
+  ('a, 'b, 'c) marked_lit HOL.equal;
+
+fun lit_of (Marked (x11, x12)) = x11
+  | lit_of (Propagated (x21, x22)) = x21;
+
+fun lits_of ls = Set.image lit_of (Set.Set ls);
+
+end; (*struct Partial_Annotated_Clausal_Logic*)
+
+structure Lattices_Big : sig
+  val max : 'a Orderings.linorder -> 'a Set.set -> 'a
+end = struct
+
+fun max A_ (Set.Set (x :: xs)) =
+  List.fold
+    (Orderings.max
+      ((Orderings.ord_preorder o Orderings.preorder_order o
+         Orderings.order_linorder)
+        A_))
+    xs x;
+
+end; (*struct Lattices_Big*)
+
+structure CDCL_W_Level : sig
+  val get_rev_level :
+    'a HOL.equal ->
+      ('a, Arith.nat, 'b) Partial_Annotated_Clausal_Logic.marked_lit list ->
+        Arith.nat -> 'a Clausal_Logic.literal -> Arith.nat
+  val get_maximum_level :
+    'a HOL.equal ->
+      ('a, Arith.nat, 'b) Partial_Annotated_Clausal_Logic.marked_lit list ->
+        'a Clausal_Logic.literal Multiset.multiset -> Arith.nat
+end = struct
+
+fun get_rev_level A_ [] uu uv = Arith.Zero_nat
+  | get_rev_level A_ (Partial_Annotated_Clausal_Logic.Marked (la, level) :: ls)
+    n l =
+    (if HOL.eq A_ (Clausal_Logic.atm_of la) (Clausal_Logic.atm_of l) then level
+      else get_rev_level A_ ls level l)
+  | get_rev_level A_ (Partial_Annotated_Clausal_Logic.Propagated (la, uw) :: ls)
+    n l =
+    (if HOL.eq A_ (Clausal_Logic.atm_of la) (Clausal_Logic.atm_of l) then n
+      else get_rev_level A_ ls n l);
+
+fun get_maximum_level A_ m d =
+  Lattices_Big.max Arith.linorder_nat
+    (Multiset.set_mset
+      (Multiset.plus_multiset (Multiset.single Arith.Zero_nat)
+        (Multiset.image_mset (get_rev_level A_ (List.rev m) Arith.Zero_nat)
+          d)));
+
+end; (*struct CDCL_W_Level*)
+
+structure Product_Type : sig
+  val equal_proda : 'a HOL.equal -> 'b HOL.equal -> 'a * 'b -> 'a * 'b -> bool
+  val equal_prod : 'a HOL.equal -> 'b HOL.equal -> ('a * 'b) HOL.equal
+end = struct
+
+fun equal_proda A_ B_ (x1, x2) (y1, y2) =
+  HOL.eq A_ x1 y1 andalso HOL.eq B_ x2 y2;
+
+fun equal_prod A_ B_ = {equal = equal_proda A_ B_} : ('a * 'b) HOL.equal;
+
+end; (*struct Product_Type*)
+
+structure DPLL_CDCL_W_Implementation : sig
+  val find_first_unused_var :
+    'a HOL.equal ->
+      ('a Clausal_Logic.literal list) list ->
+        'a Clausal_Logic.literal Set.set -> 'a Clausal_Logic.literal option
+  val find_first_unit_clause :
+    'a HOL.equal ->
+      ('a Clausal_Logic.literal list) list ->
+        ('a, 'b, 'c) Partial_Annotated_Clausal_Logic.marked_lit list ->
+          ('a Clausal_Logic.literal * 'a Clausal_Logic.literal list) option
+end = struct
+
+fun is_unit_clause_code A_ l m =
+  (case List.filter
+          (fn a =>
+            not (Set.member A_ (Clausal_Logic.atm_of a)
+                  (Set.image Clausal_Logic.atm_of
+                    (Partial_Annotated_Clausal_Logic.lits_of m))))
+          l
+    of [] => NONE
+    | [a] =>
+      (if List.list_all
+            (fn c =>
+              Set.member (Clausal_Logic.equal_literal A_)
+                (Clausal_Logic.uminus_literal c)
+                (Partial_Annotated_Clausal_Logic.lits_of m))
+            (List.remove1 (Clausal_Logic.equal_literal A_) a l)
+        then SOME a else NONE)
+    | _ :: _ :: _ => NONE);
+
+fun is_unit_clause A_ l m = is_unit_clause_code A_ l m;
+
+fun find_first_unused_var A_ (a :: l) m =
+  (case List.find
+          (fn lit =>
+            not (Set.member (Clausal_Logic.equal_literal A_) lit m) andalso
+              not (Set.member (Clausal_Logic.equal_literal A_)
+                    (Clausal_Logic.uminus_literal lit) m))
+          a
+    of NONE => find_first_unused_var A_ l m | SOME aa => SOME aa)
+  | find_first_unused_var A_ [] uu = NONE;
+
+fun find_first_unit_clause A_ (a :: l) m =
+  (case is_unit_clause A_ a m of NONE => find_first_unit_clause A_ l m
+    | SOME la => SOME (la, a))
+  | find_first_unit_clause A_ [] uu = NONE;
+
+end; (*struct DPLL_CDCL_W_Implementation*)
+
+structure CDCL_W_Implementation : sig
+  datatype cdcl_W_state_inv_from_init_state =
+    ConI of
+      ((Arith.nat, Arith.nat, (Arith.nat Clausal_Logic.literal list))
+         Partial_Annotated_Clausal_Logic.marked_lit list *
+        ((Arith.nat Clausal_Logic.literal list) list *
+          ((Arith.nat Clausal_Logic.literal list) list *
+            (Arith.nat * (Arith.nat Clausal_Logic.literal list) option))));
+  val gene : Arith.nat -> (Arith.nat Clausal_Logic.literal list) list
+  val do_all_cdcl_W_stgy :
+    cdcl_W_state_inv_from_init_state -> cdcl_W_state_inv_from_init_state
+end = struct
+
+datatype cdcl_W_state_inv =
+  Con of
+    ((Arith.nat, Arith.nat, (Arith.nat Clausal_Logic.literal list))
+       Partial_Annotated_Clausal_Logic.marked_lit list *
+      ((Arith.nat Clausal_Logic.literal list) list *
+        ((Arith.nat Clausal_Logic.literal list) list *
+          (Arith.nat * (Arith.nat Clausal_Logic.literal list) option))));
+
+datatype cdcl_W_state_inv_from_init_state =
+  ConI of
+    ((Arith.nat, Arith.nat, (Arith.nat Clausal_Logic.literal list))
+       Partial_Annotated_Clausal_Logic.marked_lit list *
+      ((Arith.nat Clausal_Logic.literal list) list *
+        ((Arith.nat Clausal_Logic.literal list) list *
+          (Arith.nat * (Arith.nat Clausal_Logic.literal list) option))));
+
+fun gene Arith.Zero_nat =
+  [[Clausal_Logic.Pos Arith.Zero_nat], [Clausal_Logic.Neg Arith.Zero_nat]]
+  | gene (Arith.Suc n) =
+    List.map (fn a => Clausal_Logic.Pos (Arith.Suc n) :: a) (gene n) @
+      List.map (fn a => Clausal_Logic.Neg (Arith.Suc n) :: a) (gene n);
+
+fun bt_cut i (Partial_Annotated_Clausal_Logic.Propagated (uu, uv) :: ls) =
+  bt_cut i ls
+  | bt_cut i (Partial_Annotated_Clausal_Logic.Marked (ka, k) :: ls) =
+    (if Arith.equal_nata k (Arith.Suc i)
+      then SOME (Partial_Annotated_Clausal_Logic.Marked (ka, k) :: ls)
+      else bt_cut i ls)
+  | bt_cut i [] = NONE;
+
+fun do_propagate_step A_ s =
+  (case s
+    of (m, (n, (u, (k, NONE)))) =>
+      (case DPLL_CDCL_W_Implementation.find_first_unit_clause A_ (n @ u) m
+        of NONE => (m, (n, (u, (k, NONE))))
+        | SOME (l, c) =>
+          (Partial_Annotated_Clausal_Logic.Propagated (l, c) :: m,
+            (n, (u, (k, NONE)))))
+    | (m, (n, (u, (k, SOME ah)))) => (m, (n, (u, (k, SOME ah)))));
+
+fun find_conflict A_ m [] = NONE
+  | find_conflict A_ m (n :: ns) =
+    (if List.list_all
+          (fn c =>
+            Set.member (Clausal_Logic.equal_literal A_)
+              (Clausal_Logic.uminus_literal c)
+              (Partial_Annotated_Clausal_Logic.lits_of m))
+          n
+      then SOME n else find_conflict A_ m ns);
+
+fun do_conflict_step A_ s =
+  (case s
+    of (m, (n, (u, (k, NONE)))) =>
+      (case find_conflict A_ m (n @ u) of NONE => (m, (n, (u, (k, NONE))))
+        | SOME a => (m, (n, (u, (k, SOME a)))))
+    | (m, (n, (u, (k, SOME ah)))) => (m, (n, (u, (k, SOME ah)))));
+
+fun do_cp_step A_ s = (do_propagate_step A_ o do_conflict_step A_) s;
+
+fun rough_state_from_init_state_of (ConI x) = x;
+
+fun id_of_I_to s = Con (rough_state_from_init_state_of s);
+
+fun rough_state_of (Con x) = x;
+
+fun do_cp_stepa s = Con (do_cp_step Arith.equal_nat (rough_state_of s));
+
+fun do_skip_step
+  (Partial_Annotated_Clausal_Logic.Propagated (l, c) :: ls,
+    (n, (u, (k, SOME d))))
+  = (if not (List.member (Clausal_Logic.equal_literal Arith.equal_nat) d
+              (Clausal_Logic.uminus_literal l)) andalso
+          not (List.null d)
+      then (ls, (n, (u, (k, SOME d))))
+      else (Partial_Annotated_Clausal_Logic.Propagated (l, c) :: ls,
+             (n, (u, (k, SOME d)))))
+  | do_skip_step ([], va) = ([], va)
+  | do_skip_step (Partial_Annotated_Clausal_Logic.Marked (vd, ve) :: vc, va) =
+    (Partial_Annotated_Clausal_Logic.Marked (vd, ve) :: vc, va)
+  | do_skip_step (v, (vb, (vd, (vf, NONE)))) = (v, (vb, (vd, (vf, NONE))));
+
+fun maximum_level_code A_ d m =
+  CDCL_W_Level.get_maximum_level A_ m (Multiset.Mset d);
+
+fun find_level_decomp A_ m [] d k = NONE
+  | find_level_decomp A_ m (l :: ls) d k =
+    let
+      val (i, j) =
+        (CDCL_W_Level.get_rev_level A_ (List.rev m) Arith.Zero_nat l,
+          maximum_level_code A_ (d @ ls) m);
+    in
+      (if Arith.equal_nata i k andalso Arith.less_nat j i then SOME (l, j)
+        else find_level_decomp A_ m ls (l :: d) k)
+    end;
+
+fun do_backtrack_step A_ (m, (n, (u, (k, SOME d)))) =
+  (case find_level_decomp A_ m d [] k of NONE => (m, (n, (u, (k, SOME d))))
+    | SOME (l, j) =>
+      (case bt_cut j m of NONE => (m, (n, (u, (k, SOME d))))
+        | SOME [] => (m, (n, (u, (k, SOME d))))
+        | SOME (Partial_Annotated_Clausal_Logic.Marked (_, _) :: ls) =>
+          (Partial_Annotated_Clausal_Logic.Propagated (l, d) :: ls,
+            (n, (d :: u, (j, NONE))))
+        | SOME (Partial_Annotated_Clausal_Logic.Propagated (_, _) :: _) =>
+          (m, (n, (u, (k, SOME d))))))
+  | do_backtrack_step A_ (v, (vb, (vd, (vf, NONE)))) =
+    (v, (vb, (vd, (vf, NONE))));
+
+fun do_resolve_step
+  (Partial_Annotated_Clausal_Logic.Propagated (l, c) :: ls,
+    (n, (u, (k, SOME d))))
+  = (if List.member (Clausal_Logic.equal_literal Arith.equal_nat) d
+          (Clausal_Logic.uminus_literal l) andalso
+          Arith.equal_nata
+            (maximum_level_code Arith.equal_nat
+              (List.remove1 (Clausal_Logic.equal_literal Arith.equal_nat)
+                (Clausal_Logic.uminus_literal l) d)
+              (Partial_Annotated_Clausal_Logic.Propagated (l, c) :: ls))
+            k
+      then (ls, (n, (u, (k, SOME (List.remdups
+                                   (Clausal_Logic.equal_literal Arith.equal_nat)
+                                   (List.remove1
+                                      (Clausal_Logic.equal_literal
+Arith.equal_nat)
+                                      l c @
+                                     List.remove1
+                                       (Clausal_Logic.equal_literal
+ Arith.equal_nat)
+                                       (Clausal_Logic.uminus_literal l) d))))))
+      else (Partial_Annotated_Clausal_Logic.Propagated (l, c) :: ls,
+             (n, (u, (k, SOME d)))))
+  | do_resolve_step ([], va) = ([], va)
+  | do_resolve_step (Partial_Annotated_Clausal_Logic.Marked (vd, ve) :: vc, va)
+    = (Partial_Annotated_Clausal_Logic.Marked (vd, ve) :: vc, va)
+  | do_resolve_step (v, (vb, (vd, (vf, NONE)))) = (v, (vb, (vd, (vf, NONE))));
+
+fun do_decide_step A_ (m, (n, (u, (k, NONE)))) =
+  (case DPLL_CDCL_W_Implementation.find_first_unused_var A_ n
+          (Partial_Annotated_Clausal_Logic.lits_of m)
+    of NONE => (m, (n, (u, (k, NONE))))
+    | SOME l =>
+      (Partial_Annotated_Clausal_Logic.Marked (l, Arith.Suc k) :: m,
+        (n, (u, (Arith.plus_nat k Arith.one_nat, NONE)))))
+  | do_decide_step A_ (v, (vb, (vd, (vf, SOME vh)))) =
+    (v, (vb, (vd, (vf, SOME vh))));
+
+fun do_other_step s =
+  let
+    val t = do_skip_step s;
+  in
+    (if not (Product_Type.equal_proda
+              (List.equal_list
+                (Partial_Annotated_Clausal_Logic.equal_marked_lit
+                  Arith.equal_nat Arith.equal_nat
+                  (List.equal_list
+                    (Clausal_Logic.equal_literal Arith.equal_nat))))
+              (Product_Type.equal_prod
+                (List.equal_list
+                  (List.equal_list
+                    (Clausal_Logic.equal_literal Arith.equal_nat)))
+                (Product_Type.equal_prod
+                  (List.equal_list
+                    (List.equal_list
+                      (Clausal_Logic.equal_literal Arith.equal_nat)))
+                  (Product_Type.equal_prod Arith.equal_nat
+                    (Option.equal_option
+                      (List.equal_list
+                        (Clausal_Logic.equal_literal Arith.equal_nat))))))
+              t s)
+      then t
+      else let
+             val u = do_resolve_step t;
+           in
+             (if not (Product_Type.equal_proda
+                       (List.equal_list
+                         (Partial_Annotated_Clausal_Logic.equal_marked_lit
+                           Arith.equal_nat Arith.equal_nat
+                           (List.equal_list
+                             (Clausal_Logic.equal_literal Arith.equal_nat))))
+                       (Product_Type.equal_prod
+                         (List.equal_list
+                           (List.equal_list
+                             (Clausal_Logic.equal_literal Arith.equal_nat)))
+                         (Product_Type.equal_prod
+                           (List.equal_list
+                             (List.equal_list
+                               (Clausal_Logic.equal_literal Arith.equal_nat)))
+                           (Product_Type.equal_prod Arith.equal_nat
+                             (Option.equal_option
+                               (List.equal_list
+                                 (Clausal_Logic.equal_literal
+                                   Arith.equal_nat))))))
+                       u t)
+               then u
+               else let
+                      val v = do_backtrack_step Arith.equal_nat u;
+                    in
+                      (if not (Product_Type.equal_proda
+                                (List.equal_list
+                                  (Partial_Annotated_Clausal_Logic.equal_marked_lit
+                                    Arith.equal_nat Arith.equal_nat
+                                    (List.equal_list
+                                      (Clausal_Logic.equal_literal
+Arith.equal_nat))))
+                                (Product_Type.equal_prod
+                                  (List.equal_list
+                                    (List.equal_list
+                                      (Clausal_Logic.equal_literal
+Arith.equal_nat)))
+                                  (Product_Type.equal_prod
+                                    (List.equal_list
+                                      (List.equal_list
+(Clausal_Logic.equal_literal Arith.equal_nat)))
+                                    (Product_Type.equal_prod Arith.equal_nat
+                                      (Option.equal_option
+(List.equal_list (Clausal_Logic.equal_literal Arith.equal_nat))))))
+                                v u)
+                        then v else do_decide_step Arith.equal_nat v)
+                    end)
+           end)
+  end;
+
+fun do_other_stepa s = Con (do_other_step (rough_state_of s));
+
+fun equal_cdcl_W_state_inv sa s =
+  Product_Type.equal_proda
+    (List.equal_list
+      (Partial_Annotated_Clausal_Logic.equal_marked_lit Arith.equal_nat
+        Arith.equal_nat
+        (List.equal_list (Clausal_Logic.equal_literal Arith.equal_nat))))
+    (Product_Type.equal_prod
+      (List.equal_list
+        (List.equal_list (Clausal_Logic.equal_literal Arith.equal_nat)))
+      (Product_Type.equal_prod
+        (List.equal_list
+          (List.equal_list (Clausal_Logic.equal_literal Arith.equal_nat)))
+        (Product_Type.equal_prod Arith.equal_nat
+          (Option.equal_option
+            (List.equal_list (Clausal_Logic.equal_literal Arith.equal_nat))))))
+    (rough_state_of sa) (rough_state_of s);
+
+fun do_full1_cp_step s =
+  let
+    val sa = do_cp_stepa s;
+  in
+    (if equal_cdcl_W_state_inv s sa then s else do_full1_cp_step sa)
+  end;
+
+fun equal_cdcl_W_state_inv_from_init_state sa s =
+  Product_Type.equal_proda
+    (List.equal_list
+      (Partial_Annotated_Clausal_Logic.equal_marked_lit Arith.equal_nat
+        Arith.equal_nat
+        (List.equal_list (Clausal_Logic.equal_literal Arith.equal_nat))))
+    (Product_Type.equal_prod
+      (List.equal_list
+        (List.equal_list (Clausal_Logic.equal_literal Arith.equal_nat)))
+      (Product_Type.equal_prod
+        (List.equal_list
+          (List.equal_list (Clausal_Logic.equal_literal Arith.equal_nat)))
+        (Product_Type.equal_prod Arith.equal_nat
+          (Option.equal_option
+            (List.equal_list (Clausal_Logic.equal_literal Arith.equal_nat))))))
+    (rough_state_from_init_state_of sa) (rough_state_from_init_state_of s);
+
+fun do_cdcl_W_stgy_step s =
+  let
+    val t = do_full1_cp_step s;
+  in
+    (if not (equal_cdcl_W_state_inv t s) then t
+      else let
+             val a = do_other_stepa t;
+           in
+             do_full1_cp_step a
+           end)
+  end;
+
+fun do_cdcl_W_stgy_stepa s =
+  ConI (rough_state_of (do_cdcl_W_stgy_step (id_of_I_to s)));
+
+fun do_all_cdcl_W_stgy s =
+  let
+    val t = do_cdcl_W_stgy_stepa s;
+  in
+    (if equal_cdcl_W_state_inv_from_init_state t s then s
+      else do_all_cdcl_W_stgy t)
+  end;
+
+end; (*struct CDCL_W_Implementation*)
+\<close>
+declare[[ML_print_depth=100]]
+ML \<open>
+open Clausal_Logic;
+open CDCL_W_Implementation;
+open Arith;
+let
+  val N = gene (Suc (Suc (Suc (((Suc Zero_nat))))))
+  val f = do_all_cdcl_W_stgy (CDCL_W_Implementation.ConI ([], (N, ([], (Zero_nat, NONE)))))
+  in
+
+  f
+end
+\<close>
+
+(*>*)
+end
